Updated the rest of the files to recent upgrade.

HybridVerifVecs/funcsets/cat2funcset.thy
@@ -1,5 +1,5 @@
 theory cat2funcset
-  imports "../hs_prelims" "Transformer_Semantics.Kleisli_Quantale"
+  imports "../hs_prelims_dyn_sys" "Transformer_Semantics.Kleisli_Quantale"
                         
 begin
 
@@ -13,12 +13,21 @@ section \<open>Verification of regular programs\<close>
 
 text \<open>First we add lemmas for computation of weakest liberal preconditions (wlps).\<close>
 
+lemma "fb\<^sub>\<F> F S = {s. F s \<subseteq> S}"
+  unfolding ffb_def map_dual_def klift_def kop_def dual_set_def
+  by(auto simp: Compl_eq_Diff_UNIV fun_eq_iff f2r_def converse_def r2f_def)
+
 lemma ffb_eta[simp]: "fb\<^sub>\<F> \<eta> X = X"
   unfolding ffb_def by(simp add: kop_def klift_def map_dual_def)
 
 lemma ffb_eq: "fb\<^sub>\<F> F X = {s. \<forall>y. y \<in> F s \<longrightarrow> y \<in> X}"
   unfolding ffb_def apply(simp add: kop_def klift_def map_dual_def)
   unfolding dual_set_def f2r_def r2f_def by auto
+
+lemma ffb_mono_ge:
+  assumes "P \<le> fb\<^sub>\<F> F R" and "R \<le> Q"
+  shows "P \<le> fb\<^sub>\<F> F Q"
+  using assms unfolding ffb_eq by auto
 
 lemma ffb_eq_univD: "fb\<^sub>\<F> F P = UNIV \<Longrightarrow> (\<forall>y. y \<in> (F x) \<longrightarrow> y \<in> P)"
 proof
@@ -48,13 +57,8 @@ lemma ffb_kcomp: "fb\<^sub>\<F> (G \<circ>\<^sub>K F) P = fb\<^sub>\<F> G (fb\<^
   unfolding ffb_def apply(simp add: kop_def klift_def map_dual_def)
   unfolding dual_set_def f2r_def r2f_def by(auto simp: kcomp_def)
 
-lemma ffb_mono_ge:
-  assumes "P \<le> fb\<^sub>\<F> F I" and "I \<le> Q"
-  shows "P \<le> fb\<^sub>\<F> F Q"
-  using assms unfolding ffb_eq by auto
-
 lemma ffb_kcomp_ge:
-  assumes "P \<le> fb\<^sub>\<F> F I" "I \<le> fb\<^sub>\<F> G Q"
+  assumes "P \<le> fb\<^sub>\<F> F R" "R \<le> fb\<^sub>\<F> G Q"
   shows "P \<le> fb\<^sub>\<F> (F \<circ>\<^sub>K G) Q"
   by(subst ffb_kcomp) (rule ffb_mono_ge[OF assms])
 
@@ -65,6 +69,10 @@ definition ifthenelse :: "'a pred \<Rightarrow> ('a \<Rightarrow> 'b set) \<Righ
   "IF P THEN X ELSE Y FI \<equiv> (\<lambda> x. if P x then X x else Y x)"
 
 lemma ffb_if_then_else:
+  "fb\<^sub>\<F> (IF T THEN X ELSE Y FI) Q = {s. T s \<longrightarrow> s \<in> fb\<^sub>\<F> X Q} \<inter> {s. \<not> T s \<longrightarrow> s \<in> fb\<^sub>\<F> Y Q}"
+  unfolding ffb_eq ifthenelse_def by auto
+
+lemma ffb_if_then_else_ge:
   assumes "P \<inter> {s. T s} \<le> fb\<^sub>\<F> X Q"
     and "P \<inter> {s. \<not> T s} \<le> fb\<^sub>\<F> Y Q"
   shows "P \<le> fb\<^sub>\<F> (IF T THEN X ELSE Y FI) Q"
@@ -72,10 +80,10 @@ lemma ffb_if_then_else:
   apply(subst (asm) ffb_eq)+
   unfolding ifthenelse_def by auto
 
-lemma ffb_if_then_elseD:
-  assumes "T x \<longrightarrow> x \<in> fb\<^sub>\<F> X Q"
-    and "\<not> T x \<longrightarrow> x \<in> fb\<^sub>\<F> Y Q"
-  shows "x \<in> fb\<^sub>\<F> (IF T THEN X ELSE Y FI) Q"
+lemma ffb_if_then_elseI:
+  assumes "T s \<longrightarrow> s \<in> fb\<^sub>\<F> X Q"
+    and "\<not> T s \<longrightarrow> s \<in> fb\<^sub>\<F> Y Q"
+  shows "s \<in> fb\<^sub>\<F> (IF T THEN X ELSE Y FI) Q"
   using assms apply(subst ffb_eq)
   apply(subst (asm) ffb_eq)+
   unfolding ifthenelse_def by auto
@@ -91,7 +99,7 @@ lemma ffb_star_induct_self: "I \<le> fb\<^sub>\<F> F I \<Longrightarrow> I \<sub
   unfolding kstar_def apply clarsimp
   using kstar_inv by blast
 
-lemma ffb_starI:
+lemma ffb_kstarI:
   assumes "P \<le> I" and "I \<le> fb\<^sub>\<F> F I" and "I \<le> Q"
   shows "P \<le> fb\<^sub>\<F> (kstar F) Q"
 proof-
@@ -100,253 +108,40 @@ proof-
   hence "P \<le> fb\<^sub>\<F> (kstar F) I"
     using assms(1) by auto
   thus ?thesis
-    using assms(3) by(subst ffb_eq, subst (asm) ffb_eq, auto)
+    using assms(3) ffb_mono_ge by blast
 qed
 
 
 section \<open>Verification of hybrid programs\<close>
 
+notation g_orbital ("(1x\<acute>=_ & _ on _ _ @ _)")
+
+abbreviation g_evol ::"(('a::banach)\<Rightarrow>'a) \<Rightarrow> 'a pred \<Rightarrow> 'a \<Rightarrow> 'a set" 
+  ("(1x\<acute>=_ & _)") where "(x\<acute>=f & G) s \<equiv> (x\<acute>=f & G on UNIV UNIV @ 0) s"
+
 subsection \<open>Verification by providing solutions\<close>
 
-abbreviation guards :: "('a \<Rightarrow> bool) \<Rightarrow> (real \<Rightarrow> 'a) \<Rightarrow> (real set) \<Rightarrow> bool" ("_ \<rhd> _ _" [70, 65] 61) 
-  where "G \<rhd> x T \<equiv> \<forall> r \<in> T. G (x r)"
-
-definition "g_orbital f T S t\<^sub>0 G s = 
-  \<Union> {{x t|t. t \<in> T \<and> G \<rhd> x {t\<^sub>0--t} }|x. x \<in> ivp_sols (\<lambda>t. f) T S t\<^sub>0 s}"
-
-lemma g_orbital_eq: "g_orbital f T S t\<^sub>0 G s =
-  {x t |t x. t \<in> T \<and> (D x = (f \<circ> x) on T) \<and> x t\<^sub>0 = s \<and> x \<in> T \<rightarrow> S \<and> G \<rhd> x {t\<^sub>0--t}}"
-  unfolding g_orbital_def ivp_sols_def by auto
-
-lemma "g_orbital f T S t\<^sub>0 G s = (\<Union> x \<in> ivp_sols (\<lambda>t. f) T S t\<^sub>0 s. {x t|t. t \<in> T \<and> G \<rhd> x {t\<^sub>0--t}})"
-  unfolding g_orbital_def ivp_sols_def by auto
-
-abbreviation g_evol ::"(('a::banach)\<Rightarrow>'a) \<Rightarrow> 'a pred \<Rightarrow> real set \<Rightarrow> 'a set \<Rightarrow> 'a \<Rightarrow> 'a set" 
-  ("(1x\<acute>=_ & _ _ _)") where "x\<acute>=f & G T S \<equiv> (\<lambda> s. g_orbital f T S 0 G s)"
-
-lemmas g_evol_def = g_orbital_eq[where t\<^sub>0 = 0]
-
-lemma g_evolI:
-  assumes "D x = (f \<circ> x) on T" "x 0 = s" "x \<in> T \<rightarrow> S"
-    and "t \<in> T" and "G \<rhd> x {0--t}"
-  shows "x t \<in> (x\<acute>=f & G T S) s"
-  using assms unfolding g_evol_def by auto
-
-lemma g_evolD:
-  assumes "s' \<in> (x\<acute>=f & G T S) s"
-  obtains x and t where "x \<in> ivp_sols (\<lambda>t. f) T UNIV 0 s" 
-  and "D x = (f \<circ> x) on T" "x 0 = s" "x \<in> T \<rightarrow> S"
-  and "x t = s'" and "t \<in> T" and "G \<rhd> x {0--t}"
-  using assms unfolding g_orbital_def ivp_sols_def by auto
-
-lemma ffb_g_evol: 
-  "fb\<^sub>\<F> (x\<acute>=f & G T S) Q = {s. \<forall>x \<in> ivp_sols (\<lambda>t. f) T S 0 s. \<forall>t\<in>T. (G \<rhd> x {0--t}) \<longrightarrow> (x t) \<in> Q}"
-  unfolding g_evol_def ffb_eq ivp_sols_def by auto
+lemma ffb_g_orbital: "fb\<^sub>\<F> (x\<acute>=f & G on T S @ t\<^sub>0) Q = 
+  {s. \<forall>x\<in>ivp_sols (\<lambda>t. f) T S t\<^sub>0 s. \<forall>t\<in>T. (G \<rhd> x (down T t)) \<longrightarrow> (x t) \<in> Q}"
+  unfolding g_orbital_eq ffb_eq ivp_sols_def by auto
 
 lemma ffb_guard_eq: 
   assumes "R = (\<lambda>s. G s \<and> Q s)"
-  shows "fb\<^sub>\<F> (x\<acute>=f & G {0..t} S) {s. R s} = fb\<^sub>\<F> (x\<acute>=f & G {0..t} S) {s. Q s}"
-  unfolding ffb_g_evol using assms by auto
+  shows "fb\<^sub>\<F> (x\<acute>=f & G on T S @ t\<^sub>0) {s. R s} = fb\<^sub>\<F> (g_orbital f G T S t\<^sub>0) {s. Q s}"
+  unfolding ffb_g_orbital using assms by auto
 
 context local_flow
 begin
 
-definition "orbit s = g_orbital f T S 0 (\<lambda>s. True) s"
-
-lemma orbit_eq[simp]: 
-  assumes "s \<in> S"
-  shows "orbit s = {\<phi> t s| t. t \<in> T}"
-  unfolding orbit_def apply safe
-  using eq_solution assms apply(subst (asm) g_orbital_def, blast)
-  unfolding g_orbital_eq by(auto intro!: has_vderiv_on_domain ivp(2) 
-      in_domain assms simp: init_time)
-
-lemma g_evol_collapses: 
-  assumes "s \<in> S"
-  shows "(x\<acute>=f & G T S) s = {\<phi> t s| t. t \<in> T \<and> G \<rhd> (\<lambda>r. \<phi> r s) {0--t}}" (is "_ = ?gorbit")
-proof(rule subset_antisym, simp_all only: subset_eq)
-  {fix s' assume "s' \<in> (x\<acute>=f & G T S) s"
-    then obtain x and t where x_ivp:"x \<in> ivp_sols (\<lambda>t. f) T S 0 s" 
-      and "x t = s'" and "t \<in> T" and guard:"G \<rhd> x {0--t}"
-      unfolding g_orbital_def by auto
-    hence obs:"\<forall>\<tau>\<in>{0..t}. x \<tau> = \<phi> \<tau> s"
-      using eq_solution[OF x_ivp _ assms] init_time
-      by (meson atLeastAtMost_iff interval_time mem_is_interval_1_I)
-    hence "G \<rhd> (\<lambda>r. \<phi> r s) {0--t}"
-      using guard by (metis \<open>s2p T t\<close> assms closed_segment_subset_domainI 
-          eq_solution init_time x_ivp) 
-    also have "\<phi> t s = x t"
-      using eq_solution[OF x_ivp \<open>t \<in> T\<close> assms] by simp
-    ultimately have "s' \<in> ?gorbit"
-      using \<open>x t = s'\<close> \<open>t \<in> T\<close> by auto}
-  thus "\<forall>s'\<in>(x\<acute>=f & G T S) s. s' \<in> ?gorbit"
-    by blast
-next
-  {fix s' assume "s' \<in> ?gorbit"
-    then obtain t where "G \<rhd> (\<lambda>r. \<phi> r s) {0--t}" and "t \<in> T" and "\<phi> t s = s'"
-      by blast
-    hence "s' \<in> (x\<acute>=f & G T S) s"
-      using assms by(auto intro!: g_evolI in_domain ivp(2) 
-          has_vderiv_on_domain simp: init_time)}
-  thus "\<forall>s'\<in>?gorbit. s' \<in> (x\<acute>=f & G T S) s"
-    by blast
-qed
-
 lemma ffb_orbit: 
   assumes "S = UNIV"
-  shows "fb\<^sub>\<F> (orbit) Q = {s. \<forall> t \<in> T. \<phi> t s \<in> Q}"
+  shows "fb\<^sub>\<F> \<gamma>\<^sup>\<phi> Q = {s. \<forall> t \<in> T. \<phi> t s \<in> Q}"
   using orbit_eq unfolding assms ffb_eq by auto
 
 lemma ffb_g_orbit: 
   assumes "S = UNIV"
-  shows "fb\<^sub>\<F> (x\<acute>=f & G T S) Q = {s. \<forall>t\<in>T. (G \<rhd> (\<lambda>r. \<phi> r s) {0--t}) \<longrightarrow> (\<phi> t s) \<in> Q}"
-  using g_evol_collapses unfolding assms ffb_eq by auto
-
-lemma ivp_sols_collapse: 
-  assumes "S = UNIV" "T = UNIV"
-  shows "ivp_sols (\<lambda>t. f) T S 0 s = {(\<lambda>t. \<phi> t s)}"
-  using in_ivp_sols eq_solution unfolding assms by auto
-
-end
-
-text\<open> The previous lemma allows us to compute wlps for known systems of ODEs. We can also implement
-a version of it as an inference rule. A simple computation of a wlp is shown immmediately after.\<close>
-
-lemma dSolution:
-  assumes "local_flow f UNIV UNIV \<phi>"
-    and "\<forall>s. s \<in> P \<longrightarrow> (\<forall> t \<in> UNIV. (G \<rhd> (\<lambda>r. \<phi> r s) {0--t}) \<longrightarrow> (\<phi> t s) \<in> Q)"
-  shows "P \<le> fb\<^sub>\<F> (x\<acute>=f & G UNIV UNIV) Q"
-  using assms by(subst local_flow.ffb_g_orbit) auto
-
-lemma ffb_line: 
-  fixes c::"'a::{heine_borel, banach}"
-  shows "fb\<^sub>\<F> (x\<acute>=(\<lambda>s. c) & G UNIV UNIV) Q = 
-    {x. \<forall> \<tau>. (G \<rhd> (\<lambda>r. x + r *\<^sub>R c) {0--\<tau>}) \<longrightarrow> (x + \<tau> *\<^sub>R c) \<in> Q}"
-  apply(subst local_flow.ffb_g_orbit[of "\<lambda>s. c" _ _ "(\<lambda> t x. x + t *\<^sub>R c)"])
-  by(auto simp: line_is_local_flow)
-
-subsection\<open> Verification with differential invariants \<close>
-
-text\<open> We derive domain specific rules of differential dynamic logic (dL). In each subsubsection, 
-we first derive the dL axioms (named below with two capital letters and ``D'' being the first one). 
-This is done mainly to prove that there are minimal requirements in Isabelle to get the dL calculus. 
-Then we prove the inference rules which are used in our verification proofs.\<close>
-
-subsubsection\<open> Differential Weakening \<close>
-
-lemma DW: "fb\<^sub>\<F> (x\<acute>=f & G {0..t} S) Q = fb\<^sub>\<F> (x\<acute>=f & G {0..t} S) {s. G s \<longrightarrow> s \<in> Q}"
-  by(auto intro: g_evolD simp: ffb_eq)
-  
-lemma dWeakening: 
-  assumes "{s. G s} \<le> Q"
-  shows "P \<le> fb\<^sub>\<F> (x\<acute>=f & G {0..t} S) Q"
-  using assms by(auto intro: g_evolD simp: le_fun_def g_evol_def ffb_eq)
-
-subsubsection\<open> Differential Cut \<close>
-
-lemma ffb_g_orbit_eq_univD:
-  assumes "fb\<^sub>\<F> (x\<acute>=f & G T S) {s. C s} = UNIV" 
-    and "\<forall> r\<in>{0..t}. x r \<in> (x\<acute>=f & G T S) s"
-  shows "\<forall>r\<in>{0..t}. C (x r)"
-proof
-  fix r assume "r \<in> {0..t}"
-  then have "x r \<in> (x\<acute>=f & G T S) s" 
-    using assms(2) by blast
-  also have "\<forall>y. y \<in> (x\<acute>=f & G T S) s \<longrightarrow> C y" 
-    using assms(1) ffb_eq_univD by fastforce
-  ultimately show "C (x r)" by blast
-qed
-
-lemma DC:
-  assumes "fb\<^sub>\<F> (x\<acute>=f & G {0..t} S) {s. C s} = UNIV"
-  shows "fb\<^sub>\<F> (x\<acute>=f & G {0..t} S) Q = fb\<^sub>\<F> (x\<acute>=f & (\<lambda>s. G s \<and> C s) {0..t} S) Q"
-proof(rule_tac f="\<lambda> x. fb\<^sub>\<F> x Q" in HOL.arg_cong, rule ext, rule subset_antisym)
-  fix s 
-  {fix s' assume "s' \<in> (x\<acute>=f & G {0..t} S) s"
-    then obtain \<tau>::real and x where x_ivp: "D x = (f \<circ> x) on {0..t}" "x 0 = s"
-      "x \<in> {0..t} \<rightarrow> S" and guard_x:"G \<rhd> x {0--\<tau>}" and "s' = x \<tau>" "\<tau> \<in> {0..t}"
-      using g_evolD[of s' "f" "{0..t}" S G s] by metis
-    from guard_x have "\<forall>r\<in>{0--\<tau>}.\<forall>\<tau>\<in>{0..r}. G (x \<tau>)"
-      by (simp add: closed_segment_eq_real_ivl)
-    also have "\<forall>\<tau>\<in>{0--\<tau>}. \<tau> \<in> {0..t}"
-      using \<open>\<tau> \<in> {0..t}\<close> by (auto simp: closed_segment_eq_real_ivl)
-    ultimately have "\<forall>\<tau>\<in>{0--\<tau>}. x \<tau> \<in> (x\<acute>=f & G {0..t} S) s"
-      using g_evolI[OF x_ivp] closed_segment_eq_real_ivl by fastforce
-    hence "C \<rhd> x {0--\<tau>}" 
-      using ffb_g_orbit_eq_univD assms by (meson ffb_eq_univD mem_Collect_eq)
-    hence "s' \<in> (x\<acute>=f & (\<lambda>s. G s \<and> C s) {0..t} S) s"
-      using g_evolI[OF x_ivp \<open>\<tau> \<in> {0..t}\<close>] guard_x \<open>s' = x \<tau>\<close> by fastforce}
-  thus "(x\<acute>=f & G {0..t} S) s \<subseteq> (x\<acute>=f & (\<lambda>s. G s \<and> C s) {0..t} S) s"
-    by blast
-next show "\<And>s. (x\<acute>=f & (\<lambda>s. G s \<and> C s) {0..t} S) s \<subseteq> (x\<acute>=f & G {0..t} S) s" 
-    by (auto simp: g_evol_def)
-qed
-
-lemma dCut:
-  assumes ffb_C:"P \<le> fb\<^sub>\<F> (x\<acute>=f & G {0..t} S) {s. C s}"
-    and ffb_Q:"P \<le> fb\<^sub>\<F> (x\<acute>=f & (\<lambda>s. G s \<and> C s) {0..t} S) Q"
-  shows "P \<le> fb\<^sub>\<F> (x\<acute>=f & G {0..t} S) Q"
-proof(subst ffb_eq, subst g_evol_def, clarsimp)
-  fix \<tau>::real and x::"real \<Rightarrow> 'a" assume "(x 0) \<in> P" and "0 \<le> \<tau>" and "\<tau> \<le> t"
-    and x_solves:"D x = (\<lambda>t. f (x t)) on {0..t}" "x \<in> {0..t} \<rightarrow> S" 
-    and guard_x:"(\<forall> r \<in> {0--\<tau>}. G (x r))"
-  hence "\<forall>r\<in>{0--\<tau>}.\<forall>\<tau>\<in>{0..r}. G (x \<tau>)"
-    by (simp add: closed_segment_eq_real_ivl)
-  hence "\<forall>r\<in>{0--\<tau>}. x r \<in> (x\<acute>=f & G {0..t} S) (x 0)"
-    using g_evolI x_solves \<open>0 \<le> \<tau>\<close> \<open>\<tau> \<le> t\<close> closed_segment_eq_real_ivl by fastforce
-  hence "\<forall>r\<in>{0--\<tau>}. C (x r)" 
-    using ffb_C \<open>(x 0) \<in> P\<close> by(subst (asm) ffb_eq, auto)
-  hence "x \<tau> \<in> (x\<acute>=f & (\<lambda>s. G s \<and> C s) {0..t} S) (x 0)"
-    using g_evolI x_solves guard_x \<open>0 \<le> \<tau>\<close> \<open>\<tau> \<le> t\<close> by fastforce
-  from this \<open>(x 0) \<in> P\<close> and ffb_Q show "(x \<tau>) \<in> Q"
-    by(subst (asm) ffb_eq) auto
-qed
-
-subsubsection\<open> Differential Invariant \<close>
-
-lemma DI_sufficiency:
-  assumes "0 \<le> t" "\<forall>s. \<exists>x. x \<in> ivp_sols (\<lambda>t. f) {0..t} S 0 s"
-  shows "fb\<^sub>\<F> (x\<acute>=f & G {0..t} S) Q \<le> fb\<^sub>\<F> (\<lambda> x. {s. s = x \<and> G s}) Q"
-  using assms apply(subst ffb_eq, subst ffb_eq, clarsimp)
-  apply(rename_tac s, erule_tac x="s" in allE, erule impE)
-  apply(simp add: g_evol_def ivp_sols_def)
-  apply(erule_tac x="s" in allE, clarify)
-  by(rule_tac x="0" in exI, rule_tac x=x in exI, auto)
-
-lemma (in local_flow) DI_necessity: (* Not true... check Bohrer formalisation *)
-  assumes "S = UNIV" "T \<subseteq> {z. z \<ge> 0}"
-  shows "fb\<^sub>\<F> (\<lambda> x. {s. s = x \<and> G s}) Q \<le> fb\<^sub>\<F> (x\<acute>=f & G T S) Q"
-  apply(subst ffb_g_orbit, simp add: assms, subst ffb_eq)
-  using assms apply(auto simp: subset_eq)
-   apply(erule_tac x=0 and P="\<lambda>t. G (\<phi> t x)" in ballE)
-  using ivp(2) apply simp_all
-  apply(erule_tac x=t and P="\<lambda>t. G (\<phi> t x)" in ballE)
-  oops
-
-definition diff_invariant :: "'a pred \<Rightarrow> (('a::real_normed_vector) \<Rightarrow> 'a) \<Rightarrow> real set \<Rightarrow> 'a set \<Rightarrow> bool" 
-("(_)/ is'_diff'_invariant'_of (_)/ along (_ _)" [70,65]61) 
-where "I is_diff_invariant_of f along T S \<equiv> 
-  (\<forall>s\<in>S. I s \<longrightarrow> (\<forall> x. x \<in> ivp_sols (\<lambda>t. f) T S 0 s \<longrightarrow> (\<forall> t \<in> T. I (x t))))"
-
-lemma invariant_to_set:
-  shows "(I is_diff_invariant_of f along T S) = 
-  (\<forall>s\<in>S. I s \<longrightarrow> (g_orbital f T S 0 (\<lambda>s. True) s) \<subseteq> {s. I s})"
-  unfolding diff_invariant_def ivp_sols_def g_orbital_eq apply safe
-   apply(erule_tac x="xa 0" in ballE)
-   apply(drule mp, simp_all)
-  apply(erule_tac x="xa 0" in ballE)
-  apply(drule mp, simp_all add: subset_eq)
-  apply(erule_tac x="xa t" in allE)
-  by(drule mp, auto)
-
-context local_flow
-begin
-
-lemma diff_invariant_eq_invariant_set:
-  "(I is_diff_invariant_of f along T S) = (\<forall>s\<in>S. \<forall>t\<in>T. I s \<longrightarrow> I (\<phi> t s))"
-  apply(subst invariant_to_set, safe)
-   apply(erule_tac x=s in ballE)
-  unfolding g_evol_collapses by auto
+  shows "fb\<^sub>\<F> (\<gamma>\<^sup>\<phi>\<^sub>G\<^sub>u\<^sub>a\<^sub>r\<^sub>d G) Q = {s. \<forall>t\<in>T. (G \<rhd> (\<lambda>r. \<phi> r s) (down T t)) \<longrightarrow> (\<phi> t s) \<in> Q}"
+  using g_orbit_eq unfolding assms ffb_eq by auto
 
 lemma invariant_set_eq_dl_invariant:
   assumes "S = UNIV"
@@ -358,107 +153,152 @@ lemma invariant_set_eq_dl_invariant:
 
 end
 
+text\<open> The previous lemma allows us to compute wlps for known systems of ODEs. We can also implement
+a version of it as an inference rule. A simple computation of a wlp is shown immediately after.\<close>
+
+lemma dSolution:
+  assumes "local_flow f T UNIV \<phi>"
+    and "\<forall>s. s \<in> P \<longrightarrow> (\<forall> t\<in>T. (G \<rhd> (\<lambda>\<tau>. \<phi> \<tau> s) (down T t)) \<longrightarrow> (\<phi> t s) \<in> Q)"
+  shows "P \<le> fb\<^sub>\<F> (x\<acute>=f & G on T UNIV @ 0) Q"
+  using assms by(subst local_flow.ffb_g_orbit) auto
+
+lemma line_is_local_flow: 
+  "0 \<in> T \<Longrightarrow> is_interval T \<Longrightarrow> open T \<Longrightarrow> local_flow (\<lambda> s. c) T UNIV (\<lambda> t s. s + t *\<^sub>R c)"
+  apply(unfold_locales, simp_all add: local_lipschitz_def lipschitz_on_def, clarsimp)
+   apply(rule_tac x=1 in exI, clarsimp, rule_tac x="1/2" in exI, simp)
+  apply(rule_tac f'1="\<lambda> s. 0" and g'1="\<lambda> s. c" in derivative_intros(191))
+  apply(rule derivative_intros, simp)+
+  by simp_all
+
+lemma ffb_line: 
+  fixes c::"'a::{heine_borel, banach}"
+  assumes "0 \<in> T" and "is_interval T" "open T"
+  shows "fb\<^sub>\<F> (x\<acute>=(\<lambda>s. c) & G on T UNIV @ 0) Q = 
+  {x. \<forall>t\<in>T. (G \<rhd> (\<lambda>\<tau>. x + \<tau> *\<^sub>R c) (down T t)) \<longrightarrow> (x + t *\<^sub>R c) \<in> Q}"
+  apply(subst local_flow.ffb_g_orbit[of "\<lambda>s. c" _ _ "(\<lambda>t x. x + t *\<^sub>R c)"])
+  using line_is_local_flow assms by auto
+
+subsection\<open> Verification with differential invariants \<close>
+
+text\<open> We derive domain specific rules of differential dynamic logic (dL). In each subsubsection, 
+we first derive the dL axioms (named below with two capital letters and ``D'' being the first one). 
+This is done mainly to prove that there are minimal requirements in Isabelle to get the dL calculus. 
+Then we prove the inference rules which are used in our verification proofs.\<close>
+
+subsubsection\<open> Differential Weakening \<close>
+
+lemma DW: "fb\<^sub>\<F> (x\<acute>=f & G on T S @ t\<^sub>0) Q = fb\<^sub>\<F> (x\<acute>=f & G on T S @ t\<^sub>0) {s. G s \<longrightarrow> s \<in> Q}"
+  by(auto intro: g_orbitalD simp: ffb_eq)
+  
+lemma dWeakening: 
+  assumes "{s. G s} \<le> Q"
+  shows "P \<le> fb\<^sub>\<F> (x\<acute>=f & G on T S @ t\<^sub>0) Q"
+  using assms by(auto intro: g_orbitalD simp: le_fun_def g_orbital_eq ffb_eq)
+
+subsubsection\<open> Differential Cut \<close>
+
+lemma ffb_g_orbital_eq_univD:
+  assumes "fb\<^sub>\<F> (x\<acute>=f & G on T S @ t\<^sub>0) {s. C s} = UNIV" 
+    and "\<forall>\<tau>\<in>(down T t). x \<tau> \<in> (x\<acute>=f & G on T S @ t\<^sub>0) s"
+  shows "\<forall>\<tau>\<in>(down T t). C (x \<tau>)"
+proof
+  fix \<tau> assume "\<tau> \<in> (down T t)"
+  hence "x \<tau> \<in> (x\<acute>=f & G on T S @ t\<^sub>0) s" 
+    using assms(2) by blast
+  also have "\<forall>y. y \<in> (x\<acute>=f & G on T S @ t\<^sub>0) s \<longrightarrow> C y" 
+    using assms(1) ffb_eq_univD by fastforce
+  ultimately show "C (x \<tau>)" by blast
+qed
+
+lemma DC:
+  assumes Thyp: "is_interval T" "t\<^sub>0 \<in> T"
+    and "fb\<^sub>\<F> (x\<acute>=f & G on T S @ t\<^sub>0) {s. C s} = UNIV"
+  shows "fb\<^sub>\<F> (x\<acute>=f & G on T S @ t\<^sub>0) Q = fb\<^sub>\<F> (x\<acute>=f & (\<lambda>s. G s \<and> C s) on T S @ t\<^sub>0) Q"
+proof(rule_tac f="\<lambda> x. fb\<^sub>\<F> x Q" in HOL.arg_cong, rule ext, rule subset_antisym)
+  fix s 
+  {fix s' assume "s' \<in> (x\<acute>=f & G on T S @ t\<^sub>0) s"
+    then obtain \<tau>::real and x where x_ivp: "D x = (f \<circ> x) on T" "x t\<^sub>0 = s"
+      "x \<in> T \<rightarrow> S" and guard_x:"G \<rhd> x (down T \<tau>)" and "s' = x \<tau>" "\<tau> \<in> T"
+      using g_orbitalD[of s' "f" G T S t\<^sub>0 s] by clarsimp metis
+    hence "\<forall>t\<in>(down T \<tau>).\<forall>\<tau>\<in>(down T t). G (x \<tau>)"
+      by (simp add: closed_segment_eq_real_ivl)
+    also have "\<forall>\<tau>\<in>(down T \<tau>). \<tau> \<in> T"
+      using \<open>\<tau> \<in> T\<close> Thyp closed_segment_subset_interval by auto
+    ultimately have "\<forall>t\<in>(down T \<tau>). x t \<in> (x\<acute>=f & G on T S @ t\<^sub>0) s"
+      using g_orbitalI[OF x_ivp] by meson
+    hence "C \<rhd> x (down T \<tau>)" 
+      using assms by (meson ffb_eq_univD mem_Collect_eq)
+    hence "s' \<in> (x\<acute>=f & (\<lambda>s. G s \<and> C s) on T S @ t\<^sub>0) s"
+      using g_orbitalI[OF x_ivp \<open>\<tau> \<in> T\<close>] guard_x \<open>s' = x \<tau>\<close> by fastforce}
+  thus "(x\<acute>=f & G on T S @ t\<^sub>0) s \<subseteq> (x\<acute>=f & (\<lambda>s. G s \<and> C s) on T S @ t\<^sub>0) s"
+    by blast
+next show "\<And>s. (x\<acute>=f & (\<lambda>s. G s \<and> C s) on T S @ t\<^sub>0) s \<subseteq> (x\<acute>=f & G on T S @ t\<^sub>0) s" 
+    by (auto simp: g_orbital_eq)
+qed
+
+lemma dCut:
+  assumes Thyp: "is_interval T" "t\<^sub>0 \<in> T"
+    and ffb_C: "P \<le> fb\<^sub>\<F> (x\<acute>=f & G on T S @ t\<^sub>0) {s. C s}"
+    and ffb_Q: "P \<le> fb\<^sub>\<F> (x\<acute>=f & (\<lambda>s. G s \<and> C s) on T S @ t\<^sub>0) Q"
+  shows "P \<le> fb\<^sub>\<F> (x\<acute>=f & G on T S @ t\<^sub>0) Q"
+proof(subst ffb_eq, subst g_orbital_eq, clarsimp)
+  fix \<tau>::real and x::"real \<Rightarrow> 'a" assume "(x t\<^sub>0) \<in> P" and "\<tau> \<in> T"
+    and x_solves:"D x = (\<lambda>t. f (x t)) on T" "x \<in> T \<rightarrow> S" 
+    and guard_x:"\<forall>t. s2p T t \<and> t \<le> \<tau> \<longrightarrow> G (x t)"
+  hence "\<forall>r\<in>(down T \<tau>). x r \<in> (x\<acute>=f & G on T S @ t\<^sub>0) (x t\<^sub>0)"
+    by (auto intro!: g_orbitalI x_solves)
+  hence "\<forall>t\<in>(down T \<tau>). C (x t)" 
+    using ffb_C \<open>(x t\<^sub>0) \<in> P\<close> by (subst (asm) ffb_eq, auto)
+  hence "x \<tau> \<in> (x\<acute>=f & (\<lambda>s. G s \<and> C s) on T S @ t\<^sub>0) (x t\<^sub>0)"
+    using guard_x \<open>\<tau> \<in> T\<close> by (auto intro!: g_orbitalI x_solves)
+  thus "(x \<tau>) \<in> Q"
+    using \<open>(x t\<^sub>0) \<in> P\<close> ffb_Q by (subst (asm) ffb_eq) auto
+qed
+
+subsubsection\<open> Differential Invariant \<close>
+
+lemma DI_sufficiency:
+  assumes "\<forall>s. \<exists>x. x \<in> ivp_sols (\<lambda>t. f) T S t\<^sub>0 s" 
+    and "t\<^sub>0 \<in> T" and "\<forall>s. \<forall>x \<in> ivp_sols (\<lambda>t. f) T S t\<^sub>0 s. \<forall>\<tau>. s2p T \<tau> \<and> \<tau> \<le> t\<^sub>0 \<longrightarrow> G (x \<tau>)"
+  shows "fb\<^sub>\<F> (x\<acute>=f & G on T S @ t\<^sub>0) Q \<le> fb\<^sub>\<F> (\<lambda> x. {s. s = x \<and> G s}) Q"
+  unfolding ffb_g_orbital using assms(1) unfolding ffb_eq apply clarsimp
+  apply(rename_tac s, erule_tac x="s" in allE, clarsimp)
+  apply(erule_tac x="x" in ballE, erule_tac x="t\<^sub>0" in ballE, erule impE)
+  using assms(3) by (simp_all add: \<open>t\<^sub>0 \<in> T\<close> ivp_solsD(2))
+
+lemma (in local_flow) DI_necessity: (* Not true... check Bohrer formalisation *)
+  assumes "S = UNIV" "T = UNIV"
+  shows "fb\<^sub>\<F> (\<lambda> x. {s. s = x \<and> G s}) Q \<le> fb\<^sub>\<F> (x\<acute>=f & G on T S @ 0) Q"
+  apply(subst ffb_g_orbit, simp add: assms, subst ffb_eq, clarsimp)
+  oops
+
 lemma dInvariant:
-  assumes "I is_diff_invariant_of f along T S" and "I\<^sub>s = {s\<in>S. I s}"
-  shows "I\<^sub>s \<le> fb\<^sub>\<F> (x\<acute>=f & G T S) I\<^sub>s"
+  assumes "I is_diff_invariant_of f along T S from t\<^sub>0" and "I\<^sub>S = {s\<in>S. I s}"
+  shows "I\<^sub>S \<le> fb\<^sub>\<F> (x\<acute>=f & G on T S @ t\<^sub>0) I\<^sub>S"
   using assms by(auto simp: diff_invariant_def ivp_sols_def ffb_eq g_orbital_eq)
 
 lemma dInvariant_converse:
-  assumes "{s\<in>S. I s} \<le> fb\<^sub>\<F> (x\<acute>=f & (\<lambda>s. True) T S) {s\<in>S. I s}"
-  shows "I is_diff_invariant_of f along T S"
+  assumes "{s\<in>S. I s} \<le> fb\<^sub>\<F> (x\<acute>=f & (\<lambda>s. True) on T S @ t\<^sub>0) {s\<in>S. I s}"
+  shows "I is_diff_invariant_of f along T S from t\<^sub>0"
   using assms unfolding invariant_to_set ffb_eq by auto
 
-lemma ffb_g_evol_le_requires:
-  assumes "\<forall>s. \<exists>x. x \<in> (ivp_sols (\<lambda>t. f) T S 0 s) \<and> G (x 0) \<and> 0 \<in> T"
-  shows "fb\<^sub>\<F> (x\<acute>=f & G T S) {s. I s} \<le> {s. I s}"
-  unfolding ffb_g_evol apply auto
-  using assms apply(erule_tac x=x in allE)
-  unfolding ivp_sols_def by auto
+lemma ffb_g_orbital_le_requires:
+  assumes "\<forall>s. \<exists>x. x \<in> (x\<acute>=f & G on T S @ t\<^sub>0) s" "\<forall>t\<in>T. t\<^sub>0 \<le> t" "t\<^sub>0\<in>T"
+  shows "fb\<^sub>\<F> (x\<acute>=f & G on T S @ t\<^sub>0) {s. I s} \<le> {s. I s}"
+  using assms unfolding ffb_eq apply clarsimp
+  apply(erule_tac x=x in allE, erule exE)
+  apply(drule g_orbitalE, clarsimp)
+  apply(frule ivp_solsD(2))
+  apply(erule_tac x="xb t\<^sub>0" in allE)
+  by(auto intro!: g_orbitalI dest: ivp_solsD)
 
 lemma dI:
-  assumes "P \<le> I" and "I \<le> fb\<^sub>\<F> (x\<acute>=f & G {0..t} S) I" and "I \<le> Q"
-  shows "P \<le> fb\<^sub>\<F> (x\<acute>=f & G {0..t} S) Q"
-  apply(rule_tac C="\<lambda>s. s \<in> I" in dCut)
+  assumes Thyp: "is_interval T" "t\<^sub>0 \<in> T"
+    and "P \<le> I" and "I \<le> fb\<^sub>\<F> (x\<acute>=f & G on T S @ t\<^sub>0) I" and "I \<le> Q"
+  shows "P \<le> fb\<^sub>\<F> (x\<acute>=f & G on T S @ t\<^sub>0) Q"
+  apply(rule_tac C="\<lambda>s. s \<in> I" in dCut[OF Thyp])
   using assms apply force
   apply(rule dWeakening)
   using assms by auto
-
-text\<open> Finally, we obtain some conditions to prove specific instances of differential invariants. \<close>
-
-named_theorems diff_invariant_rules "compilation of rules for differential invariants."
-
-lemma [diff_invariant_rules]:
-  fixes \<theta>::"'a::banach \<Rightarrow> real"
-  assumes "\<forall>x. (D x = (\<lambda>\<tau>. f (x \<tau>)) on {0..t}) \<longrightarrow> 
-  (\<forall>\<tau>\<in>{0..t}. (D (\<lambda>\<tau>. \<theta> (x \<tau>) - \<nu> (x \<tau>)) = ((*\<^sub>R) 0) on {0..\<tau>}))"
-  shows "(\<lambda>s. \<theta> s = \<nu> s) is_diff_invariant_of f along {0..t} S"
-proof(simp add: diff_invariant_def ivp_sols_def, clarsimp)
-  fix x \<tau> assume tHyp:"0 \<le> \<tau>" "\<tau> \<le> t" 
-    and x_ivp:"D x = (\<lambda>\<tau>. f (x \<tau>)) on {0..t}" "\<theta> (x 0) = \<nu> (x 0)" 
-  hence "\<forall> t \<in> {0..\<tau>}. D (\<lambda>\<tau>. \<theta> (x \<tau>) - \<nu> (x \<tau>)) \<mapsto> (\<lambda>\<tau>. \<tau> *\<^sub>R 0) at t within {0..\<tau>}" 
-    using assms by (auto simp: has_vderiv_on_def has_vector_derivative_def)
-  hence "\<exists>t\<in>{0..\<tau>}. \<theta> (x \<tau>) - \<nu> (x \<tau>) - (\<theta> (x 0) - \<nu> (x 0)) = (\<tau> - 0) \<cdot> 0" 
-    by(rule_tac mvt_very_simple) (auto simp: tHyp)
-  thus "\<theta> (x \<tau>) = \<nu> (x \<tau>)" by (simp add: x_ivp(2))
-qed
-
-lemma [diff_invariant_rules]:
-  fixes \<theta>::"'a::banach \<Rightarrow> real"
-  assumes "\<forall> x. (D x = (\<lambda>\<tau>. f (x \<tau>)) on {0..t}) \<longrightarrow> (\<forall>\<tau>\<in>{0..t}. \<theta>' (x \<tau>) \<ge> \<nu>' (x \<tau>) \<and> 
-  (D (\<lambda>\<tau>. \<theta> (x \<tau>) - \<nu> (x \<tau>)) = (\<lambda>r. \<theta>' (x r) - \<nu>' (x r)) on {0..\<tau>}))"
-  shows "(\<lambda>s. \<nu> s \<le> \<theta> s) is_diff_invariant_of f along {0..t} S"
-proof(simp add: diff_invariant_def ivp_sols_def, clarsimp)
-  fix x \<tau> assume tHyp:"0 \<le> \<tau>" "\<tau> \<le> t" 
-    and x_ivp:"D x = (\<lambda>\<tau>. f (x \<tau>)) on {0..t}" "\<nu> (x 0) \<le> \<theta> (x 0)"
-  hence primed:"\<forall> r \<in> {0..\<tau>}. (D (\<lambda>\<tau>. \<theta> (x \<tau>) - \<nu> (x \<tau>)) \<mapsto> (\<lambda>\<tau>. \<tau> *\<^sub>R (\<theta>' (x r) - \<nu>' (x r))) 
-  at r within {0..\<tau>}) \<and> \<nu>' (x r) \<le> \<theta>' (x r)" 
-    using assms by (auto simp: has_vderiv_on_def has_vector_derivative_def)
-  hence "\<exists>r\<in>{0..\<tau>}. (\<theta> (x \<tau>) - \<nu> (x \<tau>)) - (\<theta> (x 0) - \<nu> (x 0)) = 
-  (\<lambda>\<tau>. \<tau> *\<^sub>R (\<theta>' (x r) -  \<nu>' (x r))) (\<tau> - 0)" 
-    by(rule_tac mvt_very_simple) (auto simp: tHyp)
-  then obtain r where "r \<in> {0..\<tau>}" 
-    and "\<theta> (x \<tau>) - \<nu> (x \<tau>) = (\<tau> - 0) *\<^sub>R (\<theta>' (x r) -  \<nu>' (x r)) + (\<theta> (x 0) - \<nu> (x 0))" 
-    by force 
-  also have "... \<ge> 0" 
-    using tHyp(1) x_ivp(2) primed calculation(1) by auto 
-  ultimately show "\<nu> (x \<tau>) \<le> \<theta> (x \<tau>)" 
-    by simp
-qed
-
-lemma [diff_invariant_rules]:
-fixes \<theta>::"'a::banach \<Rightarrow> real"
-assumes "\<forall> x. (D x = (\<lambda>\<tau>. f (x \<tau>)) on {0..t}) \<longrightarrow> (\<forall>\<tau>\<in>{0..t}. \<theta>' (x \<tau>) \<ge> \<nu>' (x \<tau>) \<and> 
-  (D (\<lambda>\<tau>. \<theta> (x \<tau>) - \<nu> (x \<tau>)) = (\<lambda>r. \<theta>' (x r) - \<nu>' (x r)) on {0..\<tau>}))"
-shows "(\<lambda>s. \<nu> s < \<theta> s) is_diff_invariant_of f along {0..t} S"
-proof(simp add: diff_invariant_def ivp_sols_def, clarsimp)
-  fix x \<tau> assume tHyp:"0 \<le> \<tau>" "\<tau> \<le> t"
-    and x_ivp:"D x = (\<lambda>\<tau>. f (x \<tau>)) on {0..t}" "\<nu> (x 0) < \<theta> (x 0)"
-  hence primed:"\<forall> r \<in> {0..\<tau>}. ((\<lambda>\<tau>. \<theta> (x \<tau>) - \<nu> (x \<tau>)) has_derivative 
-(\<lambda>\<tau>. \<tau> *\<^sub>R  (\<theta>' (x r) -  \<nu>' (x r)))) (at r within {0..\<tau>}) \<and> \<theta>' (x r) \<ge> \<nu>' (x r)" 
-    using assms by (auto simp: has_vderiv_on_def has_vector_derivative_def)
-  hence "\<exists>r\<in>{0..\<tau>}. (\<theta> (x \<tau>) - \<nu> (x \<tau>)) - (\<theta> (x 0) - \<nu> (x 0)) = 
-  (\<lambda>\<tau>. \<tau> *\<^sub>R (\<theta>' (x r) -  \<nu>' (x r))) (\<tau> - 0)" 
-    by(rule_tac mvt_very_simple) (auto simp: tHyp)
-  then obtain r where "r \<in> {0..\<tau>}" and 
-    "\<theta> (x \<tau>) - \<nu> (x \<tau>) = (\<tau> - 0) *\<^sub>R (\<theta>' (x r) -  \<nu>' (x r)) + (\<theta> (x 0) - \<nu> (x 0))" 
-    by force 
-  also have "... > 0" 
-    using tHyp(1) x_ivp(2) primed by (metis (no_types,hide_lams) Groups.add_ac(2) add_sign_intros(1) 
-        calculation(1) diff_gt_0_iff_gt ge_iff_diff_ge_0 less_eq_real_def zero_le_scaleR_iff) 
-  ultimately show "\<nu> (x \<tau>) < \<theta> (x \<tau>)" 
-    by simp
-qed
-
-lemma [diff_invariant_rules]:
-assumes "I\<^sub>1 is_diff_invariant_of f along {0..t} S" 
-    and "I\<^sub>2 is_diff_invariant_of f along {0..t} S"
-shows "(\<lambda>s. I\<^sub>1 s \<and> I\<^sub>2 s) is_diff_invariant_of f along {0..t} S"
-  using assms unfolding diff_invariant_def by auto
-
-lemma [diff_invariant_rules]:
-assumes "I\<^sub>1 is_diff_invariant_of f along {0..t} S" 
-    and "I\<^sub>2 is_diff_invariant_of f along {0..t} S"
-shows "(\<lambda>s. I\<^sub>1 s \<or> I\<^sub>2 s) is_diff_invariant_of f along {0..t} S"
-  using assms unfolding diff_invariant_def by auto
 
 end
