HybridVerifVecs/nd_funs/cat2ndfun_examples.thy
@@ -1,15 +1,43 @@
 theory cat2ndfun_examples
-  imports cat2ndfun
+  imports "../hs_prelims_matrices" cat2ndfun
 
 begin
 
 subsection\<open> Examples \<close>
 
+no_notation Archimedean_Field.ceiling ("\<lceil>_\<rceil>")
+        and Archimedean_Field.floor_ceiling_class.floor ("\<lfloor>_\<rfloor>")
+
+lemma picard_lindeloef_linear_system:
+  fixes A::"real^'n^'n"
+  defines "L \<equiv> (real CARD('n))\<^sup>2 * (\<parallel>A\<parallel>\<^sub>m\<^sub>a\<^sub>x)"
+  shows "picard_lindeloef (\<lambda> t s. A *v s) UNIV UNIV 0"
+  apply(unfold_locales, simp_all add: local_lipschitz_def lipschitz_on_def, clarsimp)
+  apply(rule_tac x=1 in exI, clarsimp, rule_tac x="L" in exI, safe)
+  using max_norm_ge_0[of A] unfolding assms by force (rule matrix_lipschitz_constant)
+
+lemma picard_lindeloef_sq_mtx:
+  fixes A::"('n::finite) sqrd_matrix"
+  defines "L \<equiv> (real CARD('n))\<^sup>2 * (\<parallel>to_vec A\<parallel>\<^sub>m\<^sub>a\<^sub>x)"
+  shows "picard_lindeloef (\<lambda> t s. A *\<^sub>V s) UNIV UNIV 0"
+  apply(unfold_locales, simp_all add: local_lipschitz_def lipschitz_on_def, clarsimp)
+  apply(rule_tac x=1 in exI, clarsimp, rule_tac x="L" in exI, safe)
+  using max_norm_ge_0[of "to_vec A"] unfolding assms apply force
+  by transfer (rule matrix_lipschitz_constant)
+
+lemma local_flow_exp:
+  fixes A::"('n::finite) sqrd_matrix"
+  shows "local_flow ((*\<^sub>V) A) UNIV UNIV (\<lambda>t s. exp (t *\<^sub>R A) *\<^sub>V s)"
+  unfolding local_flow_def local_flow_axioms_def apply safe
+  using picard_lindeloef_sq_mtx apply blast
+  using exp_has_vderiv_on_linear[of 0] apply force
+  by(auto simp: sq_mtx_one_vec)
+
 text\<open> The examples in this subsection show different approaches for the verification of hybrid 
 systems. however, the general approach can be outlined as follows: First, we select a finite type to
 model program variables @{typ 'n}. We use this to define a vector field @{term f} of type
  @{typ "'a^'n \<Rightarrow> 'a^'n"} to model the dynamics of our system. Then we show a partial correctness 
-specification involving the evolution command @{term "([x\<acute>=f]T & G)"} either by finding a flow for 
+specification involving the evolution command @{term "(x\<acute>=f & S)"} either by finding a flow for 
 the vector field or through differential invariants.\<close>
 
 
@@ -32,7 +60,7 @@ typedef program_vars ="{''x'',''v''}"
 
 notation to_var ("\<restriction>\<^sub>V")
 
-lemma number_of_program_vars:"CARD(program_vars) = 2"
+lemma number_of_program_vars: "CARD(program_vars) = 2"
   using type_definition.card type_definition_program_vars by fastforce
 
 instance program_vars::finite
@@ -43,10 +71,10 @@ instance program_vars::finite
    apply (metis to_var_inverse UNIV_I)
   by simp
 
-lemma program_vars_univD:"(UNIV::program_vars set) = {\<restriction>\<^sub>V ''x'', \<restriction>\<^sub>V ''v''}"
+lemma program_vars_univD: "(UNIV::program_vars set) = {\<restriction>\<^sub>V ''x'', \<restriction>\<^sub>V ''v''}"
   apply auto by (metis to_str to_str_inverse insertE singletonD) 
 
-lemma program_vars_exhaust:"x = \<restriction>\<^sub>V ''x'' \<or> x = \<restriction>\<^sub>V ''v''"
+lemma program_vars_exhaust: "x = \<restriction>\<^sub>V ''x'' \<or> x = \<restriction>\<^sub>V ''v''"
   using program_vars_univD by auto
 
 abbreviation "constant_acceleration_kinematics g s \<equiv> 
@@ -62,15 +90,11 @@ lemma cnst_acc_continuous:
   by(intro tendsto_intros)
 
 lemma picard_lindeloef_cnst_acc:
-  fixes g::real assumes "0 \<le> t" and "t < 1 "
-  shows "picard_lindeloef_closed_ivl (\<lambda>t. K g) {0..t} 1 0"
-  unfolding picard_lindeloef_closed_ivl_def apply(simp add: lipschitz_on_def assms, safe)
-  apply(rule_tac t="UNIV" and f="snd" in continuous_on_compose2)
-  apply(simp_all add: cnst_acc_continuous continuous_on_snd)
-   apply(simp add: dist_vec_def L2_set_def dist_real_def)
-   apply(subst program_vars_univD, subst program_vars_univD)
-   apply(simp_all add: to_var_inject)
-  using assms by linarith
+  fixes g::real
+  shows "picard_lindeloef (\<lambda>t. K g) UNIV UNIV 0"
+  apply(unfold_locales, simp_all add: local_lipschitz_def lipschitz_on_def, clarsimp)
+  apply(rule_tac x="1/2" in exI, clarsimp, rule_tac x=1 in exI)
+  by(simp add: dist_norm norm_vec_def L2_set_def program_vars_univD to_var_inject)
 
 abbreviation "constant_acceleration_kinematics_flow g t s \<equiv> 
   (\<chi> i. if i=(\<restriction>\<^sub>V ''x'') then g \<cdot> t ^ 2/2 + s $ (\<restriction>\<^sub>V ''v'') \<cdot> t + s $ (\<restriction>\<^sub>V ''x'') 
@@ -78,26 +102,20 @@ abbreviation "constant_acceleration_kinematics_flow g t s \<equiv>
 
 notation constant_acceleration_kinematics_flow ("\<phi>\<^sub>K")
 
-term "D (\<lambda>t. \<phi>\<^sub>K g t s) = (\<lambda>t. K g (\<phi>\<^sub>K g t s)) on {0..t}"
-
-lemma local_flow_cnst_acc:
-  assumes "0 \<le> t" and "t < 1 "
-  shows "local_flow (K g) {0..t} 1 (\<phi>\<^sub>K g)"
+lemma local_flow_cnst_acc: "local_flow (K g) UNIV UNIV (\<phi>\<^sub>K g)"
   unfolding local_flow_def local_flow_axioms_def apply safe
-  using assms picard_lindeloef_cnst_acc apply blast
+  using picard_lindeloef_cnst_acc apply blast
    apply(rule has_vderiv_on_vec_lambda, clarify)
    apply(case_tac "i = \<restriction>\<^sub>V ''x''")
-  using program_vars_exhaust
-  by(auto intro!: poly_derivatives simp: to_var_inject vec_eq_iff)
+  using program_vars_exhaust by(auto intro!: poly_derivatives simp: to_var_inject vec_eq_iff)
 
 lemma single_evolution_ball:
-  fixes h::real assumes "0 \<le> t" and "t < 1" and "g < 0"
-  shows "\<lceil>\<lambda>s. 0 \<le> s $ (\<restriction>\<^sub>V ''y'') \<and> s $ (\<restriction>\<^sub>V ''y'') = h \<and> s $ (\<restriction>\<^sub>V ''v'') = 0\<rceil> 
-  \<le> wp ([x\<acute>=K g]{0..t} & (\<lambda> s. s $ (\<restriction>\<^sub>V ''y'') \<ge> 0))
-  \<lceil>\<lambda>s. 0 \<le> s $ (\<restriction>\<^sub>V ''y'') \<and> s $ (\<restriction>\<^sub>V ''y'') \<le> h\<rceil>"
-  apply(subst local_flow.wp_g_orbit[OF local_flow_cnst_acc])
-  using assms by(auto simp: mult_nonpos_nonneg)
-    (metis (full_types) less_eq_real_def program_vars_exhaust split_mult_neg_le)
+  fixes h::real assumes "g < 0" and "h \<ge> 0"
+  shows "\<lceil>\<lambda>s. s $ (\<restriction>\<^sub>V ''x'') = h \<and> s $ (\<restriction>\<^sub>V ''v'') = 0\<rceil> 
+  \<le> wp (x\<acute>=K g & (\<lambda> s. s $ (\<restriction>\<^sub>V ''x'') \<ge> 0))
+  \<lceil>\<lambda>s. 0 \<le> s $ (\<restriction>\<^sub>V ''x'') \<and> s $ (\<restriction>\<^sub>V ''x'') \<le> h\<rceil>"
+  apply(subst local_flow.wp_g_orbit[OF local_flow_cnst_acc], simp_all)
+  using assms by(auto simp: mult_nonneg_nonpos2)
 
 no_notation to_var ("\<restriction>\<^sub>V")
 
@@ -136,10 +154,10 @@ proof (induct x)
   then show ?case by auto
 qed
 
-lemma UNIV_3:"(UNIV::3 set) = {0, 1, 2}"
+lemma UNIV_3: "(UNIV::3 set) = {0, 1, 2}"
   apply safe using exhaust_3 three_eq_zero by(blast, auto)
 
-lemma sum_axis_UNIV_3[simp]:"(\<Sum>j\<in>(UNIV::3 set). axis i 1 $ j \<cdot> f j) = (f::3 \<Rightarrow> real) i"
+lemma sum_axis_UNIV_3[simp]: "(\<Sum>j\<in>(UNIV::3 set). axis i 1 $ j \<cdot> f j) = (f::3 \<Rightarrow> real) i"
   unfolding axis_def UNIV_3 apply simp
   using exhaust_3 by force
 
@@ -167,25 +185,22 @@ lemma entries_cnst_acc_matrix: "entries A = {0, 1}"
   apply (simp_all add: axis_def, safe)
   by(rule_tac x="1" in exI, simp)+
 
-lemma local_flow_cnst_acc_matrix:
-  assumes "0 \<le> t" and "t < 1/9"
-  shows "local_flow ((*v) A) {0..t} ((real CARD(3))\<^sup>2 \<cdot> (\<parallel>A\<parallel>\<^sub>m\<^sub>a\<^sub>x)) \<phi>\<^sub>A"
+lemma local_flow_cnst_acc_matrix: "local_flow ((*v) A) UNIV UNIV \<phi>\<^sub>A"
   unfolding local_flow_def local_flow_axioms_def apply safe
-    apply(rule picard_lindeloef_linear_system[where A=A and t=t])
-  using entries_cnst_acc_matrix assms apply(force, simp, force)
+     apply(rule picard_lindeloef_linear_system[where A=A], simp_all add: vec_eq_iff)
    apply(rule has_vderiv_on_vec_lambda)
    apply(auto intro!: poly_derivatives simp: matrix_vector_mult_def vec_eq_iff)
   using exhaust_3 by force
 
-text\<open> Finally, we compute the wlp of this example and use it to verify the single-evolution ball again.\<close>
+text\<open> Finally, we compute the wlp and use it to verify the single-evolution ball again.\<close>
 
-lemma single_evolution_ball_K:
-  assumes "0 \<le> t" and "t < 1/9" 
-  shows "\<lceil>\<lambda>s. 0 \<le> s $ 0 \<and> s $ 0 = h \<and> s $ 1 = 0 \<and> 0 > s $ 2\<rceil> 
-  \<le> wp ([x\<acute>=(*v) A]{0..t} & (\<lambda>s. s $ 0 \<ge> 0)) 
+lemma single_evolution_ball_K: 
+  "\<lceil>\<lambda>s. 0 \<le> s $ 0 \<and> s $ 0 = h \<and> s $ 1 = 0 \<and> 0 > s $ 2\<rceil> 
+  \<le> wp (x\<acute>=(*v) A & (\<lambda> s. s $ 0 \<ge> 0)) 
   \<lceil>\<lambda>s. 0 \<le> s $ 0 \<and> s $ 0 \<le> h\<rceil>"
-  apply(subst local_flow.wp_g_orbit[OF local_flow_cnst_acc_matrix])
-  using assms by(auto simp: mult_nonneg_nonpos2)
+  apply(subst local_flow.wp_g_orbit[of "(*v) A"])
+  using local_flow_cnst_acc_matrix apply force
+  by(auto simp: mult_nonneg_nonpos2)
 
 
 subsubsection\<open> Circular Motion \<close>
@@ -215,52 +230,41 @@ abbreviation circular_motion_matrix :: "real^2^2"
 
 notation circular_motion_matrix ("C")
 
-lemma circle_invariant:
-  shows "(\<lambda>s. r\<^sup>2 = (s $ 0)\<^sup>2 + (s $ 1)\<^sup>2) is_diff_invariant_of (*v) C along {0..t}"
-  apply(rule_tac diff_invariant_rules, clarsimp)
+lemma circle_invariant: 
+  "(\<lambda>s. r\<^sup>2 = (s $ 0)\<^sup>2 + (s $ 1)\<^sup>2) is_diff_invariant_of (*v) C along UNIV UNIV from 0"
+  apply(rule_tac diff_invariant_rules, clarsimp, simp, clarsimp)
   apply(frule_tac i="0" in has_vderiv_on_vec_nth, drule_tac i="1" in has_vderiv_on_vec_nth)
-  apply(rule_tac S="{0..t}" in has_vderiv_on_subset)
+  apply(rule_tac S="UNIV" in has_vderiv_on_subset)
   by(auto intro!: poly_derivatives simp: matrix_vector_mult_def)
 
 lemma circular_motion_invariants:
-  shows "\<lceil>\<lambda>s. r\<^sup>2 = (s $ 0)\<^sup>2 + (s $ 1)\<^sup>2\<rceil> \<le> 
-  wp ([x\<acute>=(*v) C]{0..t} & G) 
-  \<lceil>\<lambda>s. r\<^sup>2 = (s $ 0)\<^sup>2 + (s $ 1)\<^sup>2\<rceil>"
-  apply(rule_tac C="\<lambda>s. r\<^sup>2 = (s $ 0)\<^sup>2 + (s $ 1)\<^sup>2" in dCut)
-   apply(rule_tac I="\<lambda>s. r\<^sup>2 = (s $ 0)\<^sup>2 + (s $ 1)\<^sup>2" in dI)
-  using circle_invariant apply(blast, force, force)
-  by(rule dWeakening, auto)
+  "\<lceil>\<lambda>s. r\<^sup>2 = (s $ 0)\<^sup>2 + (s $ 1)\<^sup>2\<rceil> \<le> wp (x\<acute>=(*v) C & G) \<lceil>\<lambda>s. r\<^sup>2 = (s $ 0)\<^sup>2 + (s $ 1)\<^sup>2\<rceil>"
+  apply(rule_tac I="\<lambda>s. r\<^sup>2 = (s $ 0)\<^sup>2 + (s $ 1)\<^sup>2" in dInvariant)
+  using circle_invariant by auto
 
 \<comment> \<open>Proof of the same specification by providing solutions:\<close>
 
-lemma entries_circ_matrix:"entries C = {0, - 1, 1}"
+lemma entries_circ_matrix: "entries C = {0, - 1, 1}"
   apply (simp_all add: axis_def, safe)
   subgoal by(rule_tac x="0" in exI, simp)+
   subgoal by(rule_tac x="0" in exI, simp)+
   by(rule_tac x="1" in exI, simp)+
 
 abbreviation "circular_motion_matrix_flow t s \<equiv> 
-  (\<chi> i::2. if i=0 then s$0 \<cdot> cos t - s$1 \<cdot> sin t else s$0 \<cdot> sin t + s$1 \<cdot> cos t)"
+  (\<chi> i. if i= (0::2) then s$0 \<cdot> cos t - s$1 \<cdot> sin t else s$0 \<cdot> sin t + s$1 \<cdot> cos t)"
 
 notation circular_motion_matrix_flow ("\<phi>\<^sub>C")
 
-lemma local_flow_circ_mtx: 
-  assumes "0 \<le> t" and "t < 1/4" 
-  shows "local_flow ((*v) C) {0..t} ((real CARD(2))\<^sup>2 \<cdot> (\<parallel>C\<parallel>\<^sub>m\<^sub>a\<^sub>x)) \<phi>\<^sub>C"
+lemma local_flow_circ_matrix: "local_flow ((*v) C) UNIV UNIV \<phi>\<^sub>C"
   unfolding local_flow_def local_flow_axioms_def apply safe
-    apply(rule picard_lindeloef_linear_system)
-  unfolding entries_circ_matrix using assms apply(simp_all)
+  apply(rule picard_lindeloef_linear_system[where A=C], simp_all add: vec_eq_iff)
    apply(rule has_vderiv_on_vec_lambda)
   apply(force intro!: poly_derivatives simp: matrix_vector_mult_def)
   using exhaust_2 two_eq_zero by(force simp: vec_eq_iff)
 
 lemma circular_motion:
-  assumes "0 \<le> t" and "t < 1/4"
-  shows "\<lceil>\<lambda>s. r\<^sup>2 = (s $ 0)\<^sup>2 + (s $ 1)\<^sup>2\<rceil> \<le>
-   wp ([x\<acute>=(*v) C]{0..t} & G) 
-  \<lceil>\<lambda>s. r\<^sup>2 = (s $ 0)\<^sup>2 + (s $ 1)\<^sup>2\<rceil>"
-  apply(subst local_flow.wp_g_orbit[of "(*v) C" _ "(4 \<cdot> (\<parallel>C\<parallel>\<^sub>m\<^sub>a\<^sub>x))" \<phi>\<^sub>C])
-  using local_flow_circ_mtx and assms by auto
+  "\<lceil>\<lambda>s. r\<^sup>2 = (s $ 0)\<^sup>2 + (s $ 1)\<^sup>2\<rceil> \<le> wp (x\<acute>=(*v) C & G) \<lceil>\<lambda>s. r\<^sup>2 = (s $ 0)\<^sup>2 + (s $ 1)\<^sup>2\<rceil>"
+  by(subst local_flow.wp_g_orbit[OF local_flow_circ_matrix]) auto
 
 no_notation circular_motion_matrix ("C")
 
@@ -277,16 +281,20 @@ arithmetic. \<close>
 
 named_theorems bb_real_arith "real arithmetic properties for the bouncing ball."
 
-lemma [bb_real_arith]: "0 \<le> x \<Longrightarrow> 0 > g \<Longrightarrow> 2 \<cdot> g \<cdot> x = 2 \<cdot> g \<cdot> h + v \<cdot> v \<Longrightarrow> (x::real) \<le> h"
+lemma [bb_real_arith]: 
+  assumes "0 > g" and inv: "2 \<cdot> g \<cdot> x - 2 \<cdot> g \<cdot> h = v \<cdot> v"
+  shows "(x::real) \<le> h"
 proof-
-  assume "0 \<le> x" and "0 > g" and "2 \<cdot> g \<cdot> x = 2 \<cdot> g \<cdot> h + v \<cdot> v"
-  then have "v \<cdot> v = 2 \<cdot> g \<cdot> x - 2 \<cdot> g \<cdot> h \<and> 0 > g" by auto
-  hence *:"v \<cdot> v = 2 \<cdot> g \<cdot> (x - h) \<and> 0 > g \<and> v \<cdot> v \<ge> 0" 
+  have "v \<cdot> v = 2 \<cdot> g \<cdot> x - 2 \<cdot> g \<cdot> h \<and> 0 > g" 
+    using inv and \<open>0 > g\<close> by auto
+  hence obs:"v \<cdot> v = 2 \<cdot> g \<cdot> (x - h) \<and> 0 > g \<and> v \<cdot> v \<ge> 0" 
     using left_diff_distrib mult.commute by (metis zero_le_square) 
-  from this have "(v \<cdot> v)/(2 \<cdot> g) = (x - h)" by auto 
-  also from * have "(v \<cdot> v)/(2 \<cdot> g) \<le> 0"
+  hence "(v \<cdot> v)/(2 \<cdot> g) = (x - h)" 
+    by auto 
+  also from obs have "(v \<cdot> v)/(2 \<cdot> g) \<le> 0"
     using divide_nonneg_neg by fastforce 
-  ultimately have "h - x \<ge> 0" by linarith
+  ultimately have "h - x \<ge> 0" 
+    by linarith
   thus ?thesis by auto
 qed
 
@@ -294,7 +302,7 @@ lemma [bb_real_arith]:
   assumes invar: "2 \<cdot> g \<cdot> x = 2 \<cdot> g \<cdot> h + v \<cdot> v"
     and pos: "g \<cdot> \<tau>\<^sup>2 / 2 + v \<cdot> \<tau> + (x::real) = 0"
   shows "2 \<cdot> g \<cdot> h + (- (g \<cdot> \<tau>) - v) \<cdot> (- (g \<cdot> \<tau>) - v) = 0"
-and "2 \<cdot> g \<cdot> h + (g \<cdot> \<tau> \<cdot> (g \<cdot> \<tau> + v) + v \<cdot> (g \<cdot> \<tau> + v)) = 0"
+    and "2 \<cdot> g \<cdot> h + (g \<cdot> \<tau> \<cdot> (g \<cdot> \<tau> + v) + v \<cdot> (g \<cdot> \<tau> + v)) = 0"
 proof-
   from pos have "g \<cdot> \<tau>\<^sup>2  + 2 \<cdot> v \<cdot> \<tau> + 2 \<cdot> x = 0" by auto
   then have "g\<^sup>2  \<cdot> \<tau>\<^sup>2  + 2 \<cdot> g \<cdot> v \<cdot> \<tau> + 2 \<cdot> g \<cdot> x = 0"
@@ -302,14 +310,14 @@ proof-
         monoid_mult_class.power2_eq_square semiring_class.distrib_left)
   hence "g\<^sup>2 \<cdot> \<tau>\<^sup>2 + 2 \<cdot> g \<cdot> v \<cdot> \<tau> + v\<^sup>2 + 2 \<cdot> g \<cdot> h = 0"
     using invar by (simp add: monoid_mult_class.power2_eq_square) 
-  from this have *:"(g \<cdot> \<tau> + v)\<^sup>2 + 2 \<cdot> g \<cdot> h = 0"
+  hence obs: "(g \<cdot> \<tau> + v)\<^sup>2 + 2 \<cdot> g \<cdot> h = 0"
     apply(subst power2_sum) by (metis (no_types, hide_lams) Groups.add_ac(2, 3) 
         Groups.mult_ac(2, 3) monoid_mult_class.power2_eq_square nat_distrib(2))
-  hence "2 \<cdot> g \<cdot> h + (- ((g \<cdot> \<tau>) + v))\<^sup>2 = 0"
-    by (metis Groups.add_ac(2) power2_minus)
-  thus "2 \<cdot> g \<cdot> h + (- (g \<cdot> \<tau>) - v) \<cdot> (- (g \<cdot> \<tau>) - v) = 0"
+  thus "2 \<cdot> g \<cdot> h + (g \<cdot> \<tau> \<cdot> (g \<cdot> \<tau> + v) + v \<cdot> (g \<cdot> \<tau> + v)) = 0"
     by (simp add: monoid_mult_class.power2_eq_square)
-  from * show "2 \<cdot> g \<cdot> h + (g \<cdot> \<tau> \<cdot> (g \<cdot> \<tau> + v) + v \<cdot> (g \<cdot> \<tau> + v)) = 0"
+  have  "2 \<cdot> g \<cdot> h + (- ((g \<cdot> \<tau>) + v))\<^sup>2 = 0"
+    using obs by (metis Groups.add_ac(2) power2_minus)
+  thus "2 \<cdot> g \<cdot> h + (- (g \<cdot> \<tau>) - v) \<cdot> (- (g \<cdot> \<tau>) - v) = 0"
     by (simp add: monoid_mult_class.power2_eq_square)
 qed
     
@@ -334,63 +342,160 @@ proof-
 qed
 
 lemma bouncing_ball:
-  assumes "0 \<le> t" and "t < 1/9" 
-  shows "\<lceil>\<lambda>s. 0 \<le> s $ 0 \<and> s $ 0 = h \<and> s $ 1 = 0 \<and> 0 > s $ 2\<rceil> \<le> wp 
-  ((([x\<acute>=(*v) A]{0..t} & (\<lambda> s. s $ 0 \<ge> 0)) \<cdot>
+  "\<lceil>\<lambda>s. 0 \<le> s $ 0 \<and> s $ 0 = h \<and> s $ 1 = 0 \<and> 0 > s $ 2\<rceil> \<le> 
+  wp (((x\<acute>=(*v) A & (\<lambda> s. s $ 0 \<ge> 0)) \<cdot>
   (IF (\<lambda> s. s $ 0 = 0) THEN (1 ::= (\<lambda>s. - s $ 1)) ELSE \<eta>\<^sup>\<bullet> FI))\<^sup>\<star>)
   \<lceil>\<lambda>s. 0 \<le> s $ 0 \<and> s $ 0 \<le> h\<rceil>"
   apply(subst star_nd_fun.abs_eq)
-  apply(rule wp_starI[of _ "\<lceil>\<lambda>s. 0 \<le> s $ 0 \<and> 0 > s $ 2 \<and> 
-  2 \<cdot> s $ 2 \<cdot> s $ 0 = 2 \<cdot> s $ 2 \<cdot> h + (s $ 1 \<cdot> s $ 1)\<rceil>"])
+  apply(rule_tac I="\<lceil>\<lambda>s. 0 \<le> s $ 0 \<and> 0 > s $ 2 \<and> 
+  2 \<cdot> s $ 2 \<cdot> s $ 0 = 2 \<cdot> s $ 2 \<cdot> h + (s $ 1 \<cdot> s $ 1)\<rceil>" in wp_starI)
     apply(simp, simp only: fbox_mult)
    apply(subst p2ndf_ndf2p_wp[symmetric, of "(IF (\<lambda>s. s $ 0 = 0) THEN (1 ::= (\<lambda>s. - s $ 1)) ELSE \<eta>\<^sup>\<bullet> FI)"])
-   apply(subst local_flow.wp_g_orbit[of _ _ "9 \<cdot> (\<parallel>A\<parallel>\<^sub>m\<^sub>a\<^sub>x)" \<phi>\<^sub>A])
-  using local_flow_cnst_acc_matrix[OF assms] apply force
-   apply(subst ndf2p_wpD)
+   apply(subst local_flow.wp_g_orbit[OF local_flow_cnst_acc_matrix], simp, subst ndf2p_wpD)
   unfolding cond_def apply clarsimp
-   apply(transfer, simp add: kcomp_def)
-  by(auto simp: bb_real_arith)
+  by (transfer, simp add: kcomp_def) (auto simp: bb_real_arith)
+
 
 subsubsection\<open> Bouncing Ball with invariants \<close>
 
 text\<open> We prove again the bouncing ball but this time with differential invariants. \<close>
 
-lemma gravity_invariant: "(\<lambda>s. s $ 2 < 0) is_diff_invariant_of (*v) A along {0..t}"
-  apply(rule_tac \<theta>'="\<lambda>s. 0" and \<nu>'="\<lambda>s. 0" in diff_invariant_rules(3), clarsimp)
+lemma gravity_invariant: "(\<lambda>s. s $ 2 < 0) is_diff_invariant_of (*v) A along UNIV UNIV from 0"
+  apply(rule_tac \<theta>'="\<lambda>s. 0" and \<nu>'="\<lambda>s. 0" in diff_invariant_rules(3), clarsimp, simp, clarsimp)
   apply(drule_tac i="2" in has_vderiv_on_vec_nth)
-  apply(rule_tac S="{0..t}" in has_vderiv_on_subset)
+  apply(rule_tac S="UNIV" in has_vderiv_on_subset)
   by(auto intro!: poly_derivatives simp: vec_eq_iff matrix_vector_mult_def)
 
 lemma energy_conservation_invariant: 
-  "(\<lambda>s. 2 \<cdot> s$2 \<cdot> s$0 - 2 \<cdot> s$2 \<cdot> h - s$1 \<cdot> s $ 1 = 0) is_diff_invariant_of (*v) A along {0..t}"
-  apply(rule diff_invariant_rules, clarify)
+  "(\<lambda>s. 2 \<cdot> s$2 \<cdot> s$0 - 2 \<cdot> s$2 \<cdot> h - s$1 \<cdot> s $ 1 = 0) is_diff_invariant_of (*v) A along UNIV UNIV from 0"
+  apply(rule diff_invariant_rules, simp, simp, clarify)
   apply(frule_tac i="2" in has_vderiv_on_vec_nth)
   apply(frule_tac i="1" in has_vderiv_on_vec_nth)
   apply(drule_tac i="0" in has_vderiv_on_vec_nth)
-  apply(rule_tac S="{0..t}" in has_vderiv_on_subset)
+  apply(rule_tac S="UNIV" in has_vderiv_on_subset)
   by(auto intro!: poly_derivatives simp: vec_eq_iff matrix_vector_mult_def)
 
 lemma bouncing_ball_invariants: 
-  "\<lceil>\<lambda>s. 0 \<le> s $ 0 \<and> s $ 0 = h \<and> s $ 1 = 0 \<and> 0 > s $ 2\<rceil> \<le> 
-  wp ((([x\<acute>=(*v) A]{0..t} & (\<lambda> s. s $ 0 \<ge> 0)) \<cdot>
+  fixes h::real
+  defines dinv: "I \<equiv> \<lambda>s::real^3. s $ 2 < 0 \<and> 2 \<cdot> s$2 \<cdot> s$0 - 2 \<cdot> s$2 \<cdot> h - (s$1 \<cdot> s$1) = 0"
+  shows "\<lceil>\<lambda>s. 0 \<le> s $ 0 \<and> s $ 0 = h \<and> s $ 1 = 0 \<and> 0 > s $ 2\<rceil> \<le> 
+  wp (((x\<acute>=(*v) A & (\<lambda> s. s $ 0 \<ge> 0)) \<cdot>
   (IF (\<lambda> s. s $ 0 = 0) THEN (1 ::= (\<lambda>s. - s $ 1)) ELSE \<eta>\<^sup>\<bullet> FI))\<^sup>\<star>)
   \<lceil>\<lambda>s. 0 \<le> s $ 0 \<and> s $ 0 \<le> h\<rceil>"
   apply(subst star_nd_fun.abs_eq)
-  apply(rule_tac I="\<lceil>\<lambda>s. 0 \<le> s$0 \<and> 0 > s$2 \<and> 2 \<cdot> s$2 \<cdot> s$0 = 2 \<cdot> s$2 \<cdot> h + (s$1 \<cdot> s$1)\<rceil>" in wp_starI)
-    apply(simp, simp only: fbox_mult)
+  apply(rule_tac I="\<lceil>\<lambda>s. 0 \<le> s$0 \<and> I s\<rceil>" in wp_starI)
+    apply(simp add: dinv, simp only: fbox_mult)
    apply(subst p2ndf_ndf2p_wp[symmetric, of "(IF (\<lambda>s. s $ 0 = 0) THEN (1 ::= (\<lambda>s. - s $ 1)) ELSE \<eta>\<^sup>\<bullet> FI)"])
-   apply(rule dCut[where C="\<lambda> s. s $ 2 < 0"])
-    apply(rule_tac I="\<lambda> s. s $ 2 < 0" in dI)
-  using gravity_invariant apply(blast, force, force)
-   apply(rule_tac C="\<lambda> s. 2 \<cdot> s$2 \<cdot> s$0 - 2 \<cdot> s$2 \<cdot> h - s$1 \<cdot> s$1 = 0" in dCut)
-    apply(rule_tac I="\<lambda> s. 2 \<cdot> s$2 \<cdot> s$0 - 2 \<cdot> s$2 \<cdot> h - s$1 \<cdot> s$1 = 0" in dI)
-  using energy_conservation_invariant apply(blast, force, force)
-   apply(rule dWeakening, subst p2ndf_ndf2p_wp)
+  apply(rule_tac I="\<lambda>s. 0 \<le> s$0 \<and> I s" in dI, simp, simp, simp)
+    apply(subst wp_guard_eq, simp)
+    apply(rule order.trans[where b="\<lceil>I\<rceil>"], simp)
+    apply(rule dInvariant[of I], unfold dinv)
+     apply(intro diff_invariant_rules(4))
+  using gravity_invariant apply force
+  using energy_conservation_invariant apply(force, force)
+   apply(simp only: p2ndf_ndf2p_wp)
    apply(rule wp_if_then_else)
   by(auto simp: bb_real_arith le_fun_def)
 
 no_notation constant_acceleration_kinematics_matrix ("A")
 
 no_notation constant_acceleration_kinematics_matrix_flow ("\<phi>\<^sub>A")
+
+
+subsubsection\<open> Bouncing Ball with exponential solution \<close>
+
+text\<open> In our final example, we prove again the bouncing ball specification but this time we do it 
+with the general solution for linear systems.\<close>
+
+abbreviation "constant_acceleration_kinematics_sq_mtx \<equiv> 
+  sq_mtx_chi constant_acceleration_kinematics_matrix"
+
+notation constant_acceleration_kinematics_sq_mtx ("K")
+
+lemma max_norm_cnst_acc_sq_mtx: "\<parallel>to_vec K\<parallel>\<^sub>m\<^sub>a\<^sub>x = 1"
+proof-
+  have "{to_vec K $ i $ j |i j. i \<in> UNIV \<and> j \<in> UNIV} = {0, 1}"
+    apply (simp_all add: axis_def, safe)
+    by(rule_tac x="1" in exI, simp)+
+  thus ?thesis
+    by auto
+qed
+
+lemma const_acc_mtx_pow2: "(\<tau> *\<^sub>R K)\<^sup>2 = sq_mtx_chi (\<chi> i. if i=0 then \<tau>\<^sup>2 *\<^sub>R \<e> 2 else 0)"
+  unfolding monoid_mult_class.power2_eq_square apply(simp add: scaleR_sqrd_matrix_def)
+  unfolding times_sqrd_matrix_def apply(simp add: sq_mtx_chi_inject vec_eq_iff)
+  apply(simp add: matrix_matrix_mult_def)
+  unfolding UNIV_3 by(auto simp: axis_def)
+
+lemma const_acc_mtx_powN: "n > 2 \<Longrightarrow> (\<tau> *\<^sub>R K)^n = 0"
+proof(induct n)
+  case 0
+  thus ?case by simp
+next
+  case (Suc n)
+  assume IH: "2 < n \<Longrightarrow> (\<tau> *\<^sub>R K)^n = 0" and "2 < Suc n"
+  then show ?case 
+  proof(cases "n \<le> 2")
+    case True
+    hence "n = 2"
+      using \<open>2 < Suc n\<close> le_less_Suc_eq by blast 
+    hence "(\<tau> *\<^sub>R K)^(Suc n) = (\<tau> *\<^sub>R K)^3"
+      by simp
+    also have "... = (\<tau> *\<^sub>R K) \<cdot> (\<tau> *\<^sub>R K)^2"
+      by (metis (no_types, lifting) \<open>n = 2\<close> calculation power_class.power.power_Suc)
+    also have "... = (\<tau> *\<^sub>R K) \<cdot> sq_mtx_chi (\<chi> i. if i=0 then \<tau>\<^sup>2 *\<^sub>R \<e> 2 else 0)"
+      by (subst const_acc_mtx_pow2) simp
+    also have "... = 0"
+      unfolding times_sqrd_matrix_def zero_sqrd_matrix_def
+      apply(simp add: sq_mtx_chi_inject vec_eq_iff scaleR_sqrd_matrix_def)
+      apply(simp add: matrix_matrix_mult_def)
+      unfolding UNIV_3 by(auto simp: axis_def)
+    finally show ?thesis .
+  next
+    case False
+    thus ?thesis 
+      using IH by auto
+  qed
+qed
+
+lemma suminf_eq_sum:
+  fixes f :: "nat \<Rightarrow> ('a::real_normed_vector)"
+  assumes "\<And>n. n > m \<Longrightarrow> f n = 0"
+  shows "(\<Sum>n. f n) = (\<Sum>n \<le> m. f n)"
+  using assms by (meson atMost_iff finite_atMost not_le suminf_finite)
+
+lemma exp_cnst_acc_sq_mtx: "exp (\<tau> *\<^sub>R K) = ((\<tau> *\<^sub>R K)\<^sup>2/\<^sub>R 2) + (\<tau> *\<^sub>R K) + 1"
+  unfolding exp_def apply(subst suminf_eq_sum[of 2])
+  using const_acc_mtx_powN by (simp_all add: numeral_2_eq_2)
+ 
+lemma exp_cnst_acc_sq_mtx_simps:
+ "exp (\<tau> *\<^sub>R K) $$ 0 $ 0 = 1" "exp (\<tau> *\<^sub>R K) $$ 0 $ 1 = \<tau>" "exp (\<tau> *\<^sub>R K) $$ 0 $ 2 = \<tau>^2/2"
+ "exp (\<tau> *\<^sub>R K) $$ 1 $ 0 = 0" "exp (\<tau> *\<^sub>R K) $$ 1 $ 1 = 1" "exp (\<tau> *\<^sub>R K) $$ 1 $ 2 = \<tau>"
+ "exp (\<tau> *\<^sub>R K) $$ 2 $ 0 = 0" "exp (\<tau> *\<^sub>R K) $$ 2 $ 1 = 0" "exp (\<tau> *\<^sub>R K) $$ 2 $ 2 = 1"
+  unfolding exp_cnst_acc_sq_mtx const_acc_mtx_pow2 
+  by(auto simp: plus_sqrd_matrix_def scaleR_sqrd_matrix_def one_sqrd_matrix_def mat_def 
+      scaleR_vec_def axis_def plus_vec_def)
+
+lemma bouncing_ball_K: 
+  "\<lceil>\<lambda>s. 0 \<le> s $ 0 \<and> s $ 0 = h \<and> s $ 1 = 0 \<and> 0 > s $ 2\<rceil> \<le> 
+  wp (((x\<acute>=(*\<^sub>V) K & (\<lambda> s. s $ 0 \<ge> 0)) \<cdot>
+  (IF (\<lambda> s. s $ 0 = 0) THEN (1 ::= (\<lambda>s. - s $ 1)) ELSE \<eta>\<^sup>\<bullet> FI))\<^sup>\<star>)
+  \<lceil>\<lambda>s. 0 \<le> s $ 0 \<and> s $ 0 \<le> h\<rceil>"
+    apply(subst star_nd_fun.abs_eq)
+  apply(rule_tac I="\<lceil>\<lambda>s. 0 \<le> s $ 0 \<and> 0 > s $ 2 \<and> 
+  2 \<cdot> s $ 2 \<cdot> s $ 0 = 2 \<cdot> s $ 2 \<cdot> h + (s $ 1 \<cdot> s $ 1)\<rceil>" in wp_starI)
+    apply(simp, simp only: fbox_mult)
+   apply(subst p2ndf_ndf2p_wp[symmetric, of "(IF (\<lambda>s. s $ 0 = 0) THEN (1 ::= (\<lambda>s. - s $ 1)) ELSE \<eta>\<^sup>\<bullet> FI)"])
+   apply(subst local_flow.wp_g_orbit[OF local_flow_exp], simp)
+  unfolding wp_nd_fun2 apply(simp add: f2r_def cond_def plus_nd_fun_def 
+      times_nd_fun_def kcomp_def sq_mtx_vec_prod_eq)
+  unfolding UNIV_3 apply(simp add: exp_cnst_acc_sq_mtx_simps, safe)
+  subgoal for x using bb_real_arith(3)[of "x $ 2"]
+    by (simp add: add.commute mult.commute)
+  subgoal for x \<tau> using bb_real_arith(4)[where g="x $ 2" and v="x $ 1"]
+    by(simp add: add.commute mult.commute)
+  by (force simp: bb_real_arith)
+
+no_notation constant_acceleration_kinematics_sq_mtx ("K")
 
 end
