HybridVerifVecs/hs_prelims_dyn_sys.thy
@@ -1,0 +1,532 @@
+theory hs_prelims_dyn_sys
+  imports hs_prelims
+
+begin
+
+section\<open> Dynamical Systems \<close>
+
+subsection\<open> Initial value problems and orbits \<close>
+
+definition "ivp_sols f T S t\<^sub>0 s = {X |X. (D X = (\<lambda>t. f t (X t)) on T) \<and> X t\<^sub>0 = s \<and> X \<in> T \<rightarrow> S}"
+
+lemma ivp_solsI: 
+  assumes "D X = (\<lambda>t. f t (X t)) on T" "X t\<^sub>0 = s" "X \<in> T \<rightarrow> S"
+  shows "X \<in> ivp_sols f T S t\<^sub>0 s"
+  using assms unfolding ivp_sols_def by blast
+
+lemma ivp_solsD:
+  assumes "X \<in> ivp_sols f T S t\<^sub>0 s"
+  shows "D X = (\<lambda>t. f t (X t)) on T"
+    and "X t\<^sub>0 = s" and "X \<in> T \<rightarrow> S"
+  using assms unfolding ivp_sols_def by auto
+
+abbreviation guards :: "('a \<Rightarrow> bool) \<Rightarrow> (real \<Rightarrow> 'a) \<Rightarrow> (real set) \<Rightarrow> bool" ("_ \<rhd> _ _" [70, 65] 61) 
+  where "G \<rhd> X T \<equiv> \<forall>\<tau>\<in>T. G (X \<tau>)"
+
+abbreviation "down T t \<equiv> {t'\<in>T. t'\<le> t}"
+
+definition g_orbital :: "(('a::real_normed_vector) \<Rightarrow> 'a) \<Rightarrow> ('a \<Rightarrow> bool) \<Rightarrow> real set \<Rightarrow> 'a set \<Rightarrow> 
+  real \<Rightarrow> 'a \<Rightarrow> 'a set"
+  where "g_orbital f G T S t\<^sub>0 s = \<Union>{{x t|t. t \<in> T \<and> G \<rhd> x (down T t)}|x. x \<in> ivp_sols (\<lambda>t. f) T S t\<^sub>0 s}"
+
+lemma g_orbital_eq: "g_orbital f G T S t\<^sub>0 s = 
+  {x t|t x. t \<in> T \<and> (D x = (f \<circ> x) on T) \<and> x t\<^sub>0 = s \<and> x \<in> T \<rightarrow> S \<and> G \<rhd> x (down T t)}"
+  unfolding g_orbital_def ivp_sols_def by auto
+
+lemma "g_orbital f G T S t\<^sub>0 s = (\<Union>x\<in>ivp_sols (\<lambda>t. f) T S t\<^sub>0 s. {x t|t. t \<in> T \<and> G \<rhd> x (down T t)})"
+  unfolding g_orbital_def ivp_sols_def by auto
+
+lemma g_orbitalI:
+  assumes "D x = (f \<circ> x) on T" "x t\<^sub>0 = s" "x \<in> T \<rightarrow> S"
+    and "t \<in> T" and "G \<rhd> x (down T t)"
+  shows "x t \<in> g_orbital f G T S t\<^sub>0 s"
+  using assms unfolding g_orbital_eq by auto
+
+lemma g_orbitalE:
+  assumes "s' \<in> g_orbital f G T S t\<^sub>0 s"
+  shows "\<exists> x t. x \<in> ivp_sols (\<lambda>t. f) T S t\<^sub>0 s \<and> x t = s' \<and> t \<in> T \<and> G \<rhd> x (down T t)"
+  using assms unfolding g_orbital_def ivp_sols_def by auto
+
+lemma g_orbitalD:
+  assumes "s' \<in> g_orbital f G T S t\<^sub>0 s"
+  obtains x and t where "x \<in> ivp_sols (\<lambda>t. f) T S t\<^sub>0 s" 
+  and "D x = (f \<circ> x) on T" "x t\<^sub>0 = s" "x \<in> T \<rightarrow> S"
+  and "x t = s'" and "t \<in> T" and "G \<rhd> x (down T t)"
+  using assms unfolding g_orbital_def ivp_sols_def by auto
+
+
+subsection\<open> Differential Invariants \<close>
+
+definition diff_invariant :: "('a \<Rightarrow> bool) \<Rightarrow> (('a::real_normed_vector) \<Rightarrow> 'a) \<Rightarrow> real set \<Rightarrow> 
+  'a set \<Rightarrow> real \<Rightarrow> bool" ("(_)/ is'_diff'_invariant'_of (_)/ along (_ _)/ from (_)" [70,65]61) 
+  where "I is_diff_invariant_of f along T S from t\<^sub>0 \<equiv> 
+    (\<forall>s\<in>S. I s \<longrightarrow> (\<forall> x. x \<in> ivp_sols (\<lambda>t. f) T S t\<^sub>0 s \<longrightarrow> (\<forall> t \<in> T. I (x t))))"
+
+lemma invariant_to_set: "(I is_diff_invariant_of f along T S from t\<^sub>0) = 
+  (\<forall>s\<in>S. I s \<longrightarrow> (g_orbital f (\<lambda>s. True) T S t\<^sub>0 s) \<subseteq> {s. I s})"
+  unfolding diff_invariant_def ivp_sols_def g_orbital_eq apply safe
+   apply(erule_tac x="xa t\<^sub>0" in ballE)
+   apply(drule mp, simp_all)
+  apply(erule_tac x="X t\<^sub>0" in ballE)
+  apply(drule mp, simp_all add: subset_eq)
+  apply(erule_tac x="X t" in allE)
+  by(drule mp, auto)
+
+text\<open> Finally, we obtain some conditions to prove specific instances of differential invariants. \<close>
+
+named_theorems diff_invariant_rules "compilation of rules for differential invariants."
+
+lemma [diff_invariant_rules]:
+  fixes \<theta>::"'a::banach \<Rightarrow> real"
+  assumes Thyp: "is_interval T" "t\<^sub>0 \<in> T"
+    and "\<forall>x. (D x = (\<lambda>\<tau>. f (x \<tau>)) on T) \<longrightarrow> (D (\<lambda>\<tau>. \<theta> (x \<tau>) - \<nu> (x \<tau>)) = ((*\<^sub>R) 0) on T)"
+  shows "(\<lambda>s. \<theta> s = \<nu> s) is_diff_invariant_of f along T S from t\<^sub>0"
+proof(simp add: diff_invariant_def ivp_sols_def, clarsimp)
+  fix x \<tau> assume tHyp:"\<tau> \<in> T" and x_ivp:"D x = (\<lambda>\<tau>. f (x \<tau>)) on T" "\<theta> (x t\<^sub>0) = \<nu> (x t\<^sub>0)" 
+  hence obs1: "\<forall>t\<in>T. D (\<lambda>\<tau>. \<theta> (x \<tau>) - \<nu> (x \<tau>)) \<mapsto> (\<lambda>\<tau>. \<tau> *\<^sub>R 0) at t within T"
+    using assms by (auto simp: has_vderiv_on_def has_vector_derivative_def)
+  have obs2: "{t\<^sub>0--\<tau>} \<subseteq> T"
+    using closed_segment_subset_interval tHyp Thyp by blast
+  hence "D (\<lambda>\<tau>. \<theta> (x \<tau>) - \<nu> (x \<tau>)) = (\<lambda>\<tau>. \<tau> *\<^sub>R 0) on {t\<^sub>0--\<tau>}"
+    using obs1 x_ivp by (auto intro!: has_derivative_subset[OF _ obs2]
+        simp: has_vderiv_on_def has_vector_derivative_def)
+  then obtain t where "t \<in> {t\<^sub>0--\<tau>}" and "\<theta> (x \<tau>) - \<nu> (x \<tau>) - (\<theta> (x t\<^sub>0) - \<nu> (x t\<^sub>0)) = (\<tau> - t\<^sub>0) * t *\<^sub>R 0"
+    using mvt_very_simple_closed_segmentE by blast
+  thus "\<theta> (x \<tau>) = \<nu> (x \<tau>)" 
+    by (simp add: x_ivp(2))
+qed
+
+lemma [diff_invariant_rules]:
+  fixes \<theta>::"'a::banach \<Rightarrow> real"
+  assumes Thyp: "is_interval T" "t\<^sub>0 \<in> T"
+    and "\<forall> x. (D x = (\<lambda>\<tau>. f (x \<tau>)) on T) \<longrightarrow> (\<forall>\<tau>\<in>T. (\<tau> > t\<^sub>0 \<longrightarrow> \<theta>' (x \<tau>) \<ge> \<nu>' (x \<tau>)) \<and> 
+(\<tau> < t\<^sub>0 \<longrightarrow> \<theta>' (x \<tau>) \<le> \<nu>' (x \<tau>))) \<and> (D (\<lambda>\<tau>. \<theta> (x \<tau>) - \<nu> (x \<tau>)) = (\<lambda>\<tau>. \<theta>' (x \<tau>) - \<nu>' (x \<tau>)) on T)"
+  shows "(\<lambda>s. \<nu> s \<le> \<theta> s) is_diff_invariant_of f along T S from t\<^sub>0"
+proof(simp add: diff_invariant_def ivp_sols_def, clarsimp)
+  fix x \<tau> assume "\<tau> \<in> T" and x_ivp:"D x = (\<lambda>\<tau>. f (x \<tau>)) on T" "\<nu> (x t\<^sub>0) \<le> \<theta> (x t\<^sub>0)"
+  {assume "\<tau> \<noteq> t\<^sub>0"
+  hence primed: "\<And>\<tau>. \<tau> \<in> T \<Longrightarrow> \<tau> > t\<^sub>0 \<Longrightarrow> \<theta>' (x \<tau>) \<ge> \<nu>' (x \<tau>)" 
+    "\<And>\<tau>. \<tau> \<in> T \<Longrightarrow> \<tau> < t\<^sub>0 \<Longrightarrow> \<theta>' (x \<tau>) \<le> \<nu>' (x \<tau>)"
+    using x_ivp assms by auto
+  have obs1: "\<forall>t\<in>T. D (\<lambda>\<tau>. \<theta> (x \<tau>) - \<nu> (x \<tau>)) \<mapsto> (\<lambda>\<tau>. \<tau> *\<^sub>R (\<theta>' (x t) - \<nu>' (x t))) at t within T"
+    using assms x_ivp by (auto simp: has_vderiv_on_def has_vector_derivative_def)
+  have obs2: "{t\<^sub>0<--<\<tau>} \<subseteq> T" "{t\<^sub>0--\<tau>} \<subseteq> T"
+    using \<open>\<tau> \<in> T\<close> Thyp \<open>\<tau> \<noteq> t\<^sub>0\<close> by (auto simp: convex_contains_open_segment 
+        is_interval_convex_1 closed_segment_subset_interval)
+  hence "D (\<lambda>\<tau>. \<theta> (x \<tau>) - \<nu> (x \<tau>)) = (\<lambda>\<tau>. \<theta>' (x \<tau>) - \<nu>' (x \<tau>)) on {t\<^sub>0--\<tau>}"
+    using obs1 x_ivp by (auto intro!: has_derivative_subset[OF _ obs2(2)]
+        simp: has_vderiv_on_def has_vector_derivative_def)
+  then obtain t where "t \<in> {t\<^sub>0<--<\<tau>}" and
+    "(\<theta> (x \<tau>) - \<nu> (x \<tau>)) - (\<theta> (x t\<^sub>0) - \<nu> (x t\<^sub>0)) = (\<lambda>\<tau>. \<tau> * (\<theta>' (x t) -  \<nu>' (x t))) (\<tau> - t\<^sub>0)"
+    using mvt_simple_closed_segmentE \<open>\<tau> \<noteq> t\<^sub>0\<close> by blast
+  hence mvt: "\<theta> (x \<tau>) - \<nu> (x \<tau>) = (\<tau> - t\<^sub>0) * (\<theta>' (x t) -  \<nu>' (x t)) + (\<theta> (x t\<^sub>0) - \<nu> (x t\<^sub>0))" 
+    by force
+  have  "\<tau> > t\<^sub>0 \<Longrightarrow> t > t\<^sub>0" "\<not> t\<^sub>0 \<le> \<tau> \<Longrightarrow> t < t\<^sub>0" "t \<in> T"
+    using \<open>t \<in> {t\<^sub>0<--<\<tau>}\<close> obs2 unfolding open_segment_eq_real_ivl by auto
+  moreover have "t > t\<^sub>0 \<Longrightarrow> (\<theta>' (x t) -  \<nu>' (x t)) \<ge> 0" "t < t\<^sub>0 \<Longrightarrow> (\<theta>' (x t) -  \<nu>' (x t)) \<le> 0"
+    using primed(1,2)[OF \<open>t \<in> T\<close>] by auto
+  ultimately have "(\<tau> - t\<^sub>0) * (\<theta>' (x t) -  \<nu>' (x t)) \<ge> 0"
+    apply(case_tac "\<tau> \<ge> t\<^sub>0") by (force, auto simp: split_mult_pos_le)
+  hence "(\<tau> - t\<^sub>0) * (\<theta>' (x t) -  \<nu>' (x t)) + (\<theta> (x t\<^sub>0) - \<nu> (x t\<^sub>0)) \<ge> 0" 
+    using  x_ivp(2) by auto
+  hence "\<nu> (x \<tau>) \<le> \<theta> (x \<tau>)" 
+    using mvt by simp}
+  thus "\<nu> (x \<tau>) \<le> \<theta> (x \<tau>)"
+    using x_ivp by blast
+qed
+
+lemma [diff_invariant_rules]:
+  fixes \<theta>::"'a::banach \<Rightarrow> real"
+  assumes Thyp: "is_interval T" "t\<^sub>0 \<in> T"
+    and "\<forall> x. (D x = (\<lambda>\<tau>. f (x \<tau>)) on T) \<longrightarrow> (\<forall>\<tau>\<in>T. (\<tau> > t\<^sub>0 \<longrightarrow> \<theta>' (x \<tau>) \<ge> \<nu>' (x \<tau>)) \<and> 
+(\<tau> < t\<^sub>0 \<longrightarrow> \<theta>' (x \<tau>) \<le> \<nu>' (x \<tau>))) \<and> (D (\<lambda>\<tau>. \<theta> (x \<tau>) - \<nu> (x \<tau>)) = (\<lambda>\<tau>. \<theta>' (x \<tau>) - \<nu>' (x \<tau>)) on T)"
+  shows "(\<lambda>s. \<nu> s < \<theta> s) is_diff_invariant_of f along T S from t\<^sub>0"
+proof(simp add: diff_invariant_def ivp_sols_def, clarsimp)
+  fix x \<tau> assume "\<tau> \<in> T" and x_ivp:"D x = (\<lambda>\<tau>. f (x \<tau>)) on T" "\<nu> (x t\<^sub>0) < \<theta> (x t\<^sub>0)"
+  {assume "\<tau> \<noteq> t\<^sub>0"
+  hence primed: "\<And>\<tau>. \<tau> \<in> T \<Longrightarrow> \<tau> > t\<^sub>0 \<Longrightarrow> \<theta>' (x \<tau>) \<ge> \<nu>' (x \<tau>)" 
+    "\<And>\<tau>. \<tau> \<in> T \<Longrightarrow> \<tau> < t\<^sub>0 \<Longrightarrow> \<theta>' (x \<tau>) \<le> \<nu>' (x \<tau>)"
+    using x_ivp assms by auto
+  have obs1: "\<forall>t\<in>T. D (\<lambda>\<tau>. \<theta> (x \<tau>) - \<nu> (x \<tau>)) \<mapsto> (\<lambda>\<tau>. \<tau> *\<^sub>R (\<theta>' (x t) - \<nu>' (x t))) at t within T"
+    using assms x_ivp by (auto simp: has_vderiv_on_def has_vector_derivative_def)
+  have obs2: "{t\<^sub>0<--<\<tau>} \<subseteq> T" "{t\<^sub>0--\<tau>} \<subseteq> T"
+    using \<open>\<tau> \<in> T\<close> Thyp \<open>\<tau> \<noteq> t\<^sub>0\<close> by (auto simp: convex_contains_open_segment 
+        is_interval_convex_1 closed_segment_subset_interval)
+  hence "D (\<lambda>\<tau>. \<theta> (x \<tau>) - \<nu> (x \<tau>)) = (\<lambda>\<tau>. \<theta>' (x \<tau>) - \<nu>' (x \<tau>)) on {t\<^sub>0--\<tau>}"
+    using obs1 x_ivp by (auto intro!: has_derivative_subset[OF _ obs2(2)]
+        simp: has_vderiv_on_def has_vector_derivative_def)
+  then obtain t where "t \<in> {t\<^sub>0<--<\<tau>}" and
+    "(\<theta> (x \<tau>) - \<nu> (x \<tau>)) - (\<theta> (x t\<^sub>0) - \<nu> (x t\<^sub>0)) = (\<lambda>\<tau>. \<tau> * (\<theta>' (x t) -  \<nu>' (x t))) (\<tau> - t\<^sub>0)"
+    using mvt_simple_closed_segmentE \<open>\<tau> \<noteq> t\<^sub>0\<close> by blast
+  hence mvt: "\<theta> (x \<tau>) - \<nu> (x \<tau>) = (\<tau> - t\<^sub>0) * (\<theta>' (x t) -  \<nu>' (x t)) + (\<theta> (x t\<^sub>0) - \<nu> (x t\<^sub>0))" 
+    by force
+  have  "\<tau> > t\<^sub>0 \<Longrightarrow> t > t\<^sub>0" "\<not> t\<^sub>0 \<le> \<tau> \<Longrightarrow> t < t\<^sub>0" "t \<in> T"
+    using \<open>t \<in> {t\<^sub>0<--<\<tau>}\<close> obs2 unfolding open_segment_eq_real_ivl by auto
+  moreover have "t > t\<^sub>0 \<Longrightarrow> (\<theta>' (x t) -  \<nu>' (x t)) \<ge> 0" "t < t\<^sub>0 \<Longrightarrow> (\<theta>' (x t) -  \<nu>' (x t)) \<le> 0"
+    using primed(1,2)[OF \<open>t \<in> T\<close>] by auto
+  ultimately have "(\<tau> - t\<^sub>0) * (\<theta>' (x t) -  \<nu>' (x t)) \<ge> 0"
+    apply(case_tac "\<tau> \<ge> t\<^sub>0") by (force, auto simp: split_mult_pos_le)
+  hence "(\<tau> - t\<^sub>0) * (\<theta>' (x t) -  \<nu>' (x t)) + (\<theta> (x t\<^sub>0) - \<nu> (x t\<^sub>0)) > 0" 
+    using x_ivp(2) by auto
+  hence "\<nu> (x \<tau>) < \<theta> (x \<tau>)" 
+    using mvt by simp}
+  thus "\<nu> (x \<tau>) < \<theta> (x \<tau>)"
+    using x_ivp by blast
+qed
+
+lemma [diff_invariant_rules]:
+assumes "I\<^sub>1 is_diff_invariant_of f along T S from t\<^sub>0" 
+    and "I\<^sub>2 is_diff_invariant_of f along T S from t\<^sub>0"
+shows "(\<lambda>s. I\<^sub>1 s \<and> I\<^sub>2 s) is_diff_invariant_of f along T S from t\<^sub>0"
+  using assms unfolding diff_invariant_def by auto
+
+lemma [diff_invariant_rules]:
+assumes "I\<^sub>1 is_diff_invariant_of f along T S from t\<^sub>0" 
+    and "I\<^sub>2 is_diff_invariant_of f along T S from t\<^sub>0"
+shows "(\<lambda>s. I\<^sub>1 s \<or> I\<^sub>2 s) is_diff_invariant_of f along T S from t\<^sub>0"
+  using assms unfolding diff_invariant_def by auto
+
+
+subsection\<open> Picard-Lindeloef \<close>
+
+text\<open> The next locale makes explicit the conditions for applying the Picard-Lindeloef theorem. This
+guarantees a unique solution for every initial value problem represented with a vector field 
+@{term f} and an initial time @{term t\<^sub>0}. It is mostly a simplified reformulation of the approach 
+taken by the people who created the Ordinary Differential Equations entry in the AFP. \<close>
+
+locale picard_lindeloef =
+  fixes f::"real \<Rightarrow> ('a::{heine_borel,banach}) \<Rightarrow> 'a" and T::"real set" and S::"'a set" and t\<^sub>0::real
+  assumes init_time: "t\<^sub>0 \<in> T"
+    and cont_vec_field: "\<forall>s \<in> S. continuous_on T (\<lambda>t. f t s)"
+    and lipschitz_vec_field: "local_lipschitz T S f"
+    and interval_time: "is_interval T"
+    and open_domain: "open T" "open S"
+begin
+
+sublocale ll_on_open_it T f S t\<^sub>0
+  by (unfold_locales) (auto simp: cont_vec_field lipschitz_vec_field interval_time open_domain) 
+
+lemmas subintervalI = closed_segment_subset_domain
+
+lemma subintervalD:
+  assumes "{t\<^sub>1--t\<^sub>2} \<subseteq> T"
+  shows "t\<^sub>1 \<in> T" and "t\<^sub>2 \<in> T"
+  using assms by auto
+
+lemma csols_eq: "csols t\<^sub>0 s = {(X, t). t \<in> T \<and>  X \<in> ivp_sols f {t\<^sub>0--t} S t\<^sub>0 s}"
+  unfolding ivp_sols_def csols_def solves_ode_def using subintervalI[OF init_time] by auto
+
+abbreviation "ex_ivl s \<equiv> existence_ivl t\<^sub>0 s"
+
+lemma unique_solution:
+  assumes xivp: "D X = (\<lambda>t. f t (X t)) on {t\<^sub>0--t}" "X t\<^sub>0 = s" "X \<in> {t\<^sub>0--t} \<rightarrow> S" and "t \<in> T"
+    and yivp: "D Y = (\<lambda>t. f t (Y t)) on {t\<^sub>0--t}" "Y t\<^sub>0 = s" "Y \<in> {t\<^sub>0--t} \<rightarrow> S" and "s \<in> S" 
+  shows "X t = Y t"
+proof-
+  have "(X, t) \<in> csols t\<^sub>0 s"
+    using xivp \<open>t \<in> T\<close> unfolding csols_eq ivp_sols_def by auto
+  hence ivl_fact: "{t\<^sub>0--t} \<subseteq> ex_ivl s"
+    unfolding existence_ivl_def by auto
+  have obs: "\<And>z T'. t\<^sub>0 \<in> T' \<and> is_interval T' \<and> T' \<subseteq> ex_ivl s \<and> (z solves_ode f) T' S \<Longrightarrow> 
+  z t\<^sub>0 = flow t\<^sub>0 s t\<^sub>0 \<Longrightarrow> (\<forall>t\<in>T'. z t = flow t\<^sub>0 s t)"
+    using flow_usolves_ode[OF init_time \<open>s \<in> S\<close>] unfolding usolves_ode_from_def by blast
+  have "\<forall>\<tau>\<in>{t\<^sub>0--t}. X \<tau> = flow t\<^sub>0 s \<tau>"
+    using obs[of "{t\<^sub>0--t}" X] xivp ivl_fact flow_initial_time[OF init_time  \<open>s \<in> S\<close>] 
+    unfolding solves_ode_def by simp
+  also have "\<forall>\<tau>\<in>{t\<^sub>0--t}. Y \<tau> = flow t\<^sub>0 s \<tau>"
+    using obs[of "{t\<^sub>0--t}" Y] yivp ivl_fact flow_initial_time[OF init_time  \<open>s \<in> S\<close>] 
+    unfolding solves_ode_def by simp
+  ultimately show "X t = Y t"
+    by auto
+qed
+
+lemma solution_eq_flow:
+  assumes xivp: "D X = (\<lambda>t. f t (X t)) on ex_ivl s" "X t\<^sub>0 = s" "X \<in> ex_ivl s \<rightarrow> S" 
+    and "t \<in> ex_ivl s" and "s \<in> S" 
+  shows "X t = flow t\<^sub>0 s t"
+proof-
+  have obs: "\<And>z T'. t\<^sub>0 \<in> T' \<and> is_interval T' \<and> T' \<subseteq> ex_ivl s \<and> (z solves_ode f) T' S \<Longrightarrow> 
+  z t\<^sub>0 = flow t\<^sub>0 s t\<^sub>0 \<Longrightarrow> (\<forall>t\<in>T'. z t = flow t\<^sub>0 s t)"
+    using flow_usolves_ode[OF init_time \<open>s \<in> S\<close>] unfolding usolves_ode_from_def by blast
+  have "\<forall>\<tau>\<in>ex_ivl s. X \<tau> = flow t\<^sub>0 s \<tau>"
+    using obs[of "ex_ivl s" X] existence_ivl_initial_time[OF init_time \<open>s \<in> S\<close>]
+      xivp flow_initial_time[OF init_time \<open>s \<in> S\<close>] unfolding solves_ode_def by simp
+  thus "X t = flow t\<^sub>0 s t"
+    by (auto simp: \<open>t \<in> ex_ivl s\<close>)
+qed
+
+end
+
+subsection\<open> Flows for ODEs \<close>
+
+text\<open> This locale is a particular case of the previous one. It makes the unique solution for initial 
+value problems explicit, it restricts the vector field to reflect autonomous systems (those that do 
+not depend explicitly on time), and it sets the initial time equal to 0. This is the first step 
+towards formalizing the flow of a differential equation, i.e. the function that maps every point to 
+the unique trajectory tangent to the vector field. \<close>
+
+locale local_flow = picard_lindeloef "(\<lambda> t. f)" T S 0 
+  for f::"('a::{heine_borel,banach}) \<Rightarrow> 'a" and T S L +
+  fixes \<phi> :: "real \<Rightarrow> 'a \<Rightarrow> 'a"
+  assumes ivp:"\<And> t s. t \<in> T \<Longrightarrow> s \<in> S \<Longrightarrow> (D (\<lambda>t. \<phi> t s) = (\<lambda>t. f (\<phi> t s)) on {0--t})"
+              "\<And> s. s \<in> S \<Longrightarrow> \<phi> 0 s = s"
+              "\<And> t s. t \<in> T \<Longrightarrow> s \<in> S \<Longrightarrow> (\<lambda>t. \<phi> t s) \<in> {0--t} \<rightarrow> S"
+begin
+
+abbreviation g_orbit :: "('a \<Rightarrow> bool) \<Rightarrow> 'a \<Rightarrow> 'a set" ("\<gamma>\<^sup>\<phi>\<^sub>G\<^sub>u\<^sub>a\<^sub>r\<^sub>d")
+  where "\<gamma>\<^sup>\<phi>\<^sub>G\<^sub>u\<^sub>a\<^sub>r\<^sub>d G s \<equiv> g_orbital f G T S 0 s"
+
+definition "orbit s = \<gamma>\<^sup>\<phi>\<^sub>G\<^sub>u\<^sub>a\<^sub>r\<^sub>d (\<lambda>s. True) s"
+
+notation orbit ("\<gamma>\<^sup>\<phi>")
+
+lemma in_ivp_sols_ivl: 
+  assumes "t \<in> T" "s \<in> S"
+  shows "(\<lambda>t. \<phi> t s) \<in> ivp_sols (\<lambda>t. f) {0--t} S 0 s"
+  apply(rule ivp_solsI)
+  using ivp assms by auto
+
+lemma ex_ivl_eq:
+  assumes "s \<in> S"
+  shows "ex_ivl s = T"
+  using existence_ivl_subset[of s] apply safe
+  unfolding existence_ivl_def csols_eq 
+  using in_ivp_sols_ivl[OF _ assms] by blast
+
+lemma in_domain:
+  assumes "s \<in> S"
+  shows "(\<lambda>t. \<phi> t s) \<in> T \<rightarrow> S"
+  unfolding ex_ivl_eq[symmetric] existence_ivl_def
+  using local.mem_existence_ivl_subset ivp(3)[OF _ assms] by blast
+
+lemma has_derivative_on_open1: 
+  assumes  "t > 0" "t \<in> T" "s \<in> S"
+  obtains B where "t \<in> B" and "open B" and "B \<subseteq> T"
+    and "D (\<lambda>\<tau>. \<phi> \<tau> s) \<mapsto> (\<lambda>\<tau>. \<tau> *\<^sub>R f (\<phi> t s)) at t within B" 
+proof-
+  obtain r::real where rHyp: "r > 0" "ball t r \<subseteq> T"
+    using open_contains_ball_eq open_domain(1) \<open>t \<in> T\<close> by blast
+  moreover have "t + r/2 > 0"
+    using \<open>r > 0\<close> \<open>t > 0\<close> by auto
+  moreover have "{0--t} \<subseteq> T" 
+    using subintervalI[OF init_time \<open>t \<in> T\<close>] .
+  ultimately have subs: "{0<--<t + r/2} \<subseteq> T"
+    unfolding abs_le_eq abs_le_eq real_ivl_eqs[OF \<open>t > 0\<close>] real_ivl_eqs[OF \<open>t + r/2 > 0\<close>] 
+    by clarify (case_tac "t < x", simp_all add: cball_def ball_def dist_norm subset_eq field_simps)
+  have "t + r/2 \<in> T"
+    using rHyp unfolding real_ivl_eqs[OF rHyp(1)] by (simp add: subset_eq)
+  hence "{0--t + r/2} \<subseteq> T"
+    using subintervalI[OF init_time] by blast
+  hence "(D (\<lambda>t. \<phi> t s) = (\<lambda>t. f (\<phi> t s)) on {0--(t + r/2)})"
+    using ivp(1)[OF _ \<open>s \<in> S\<close>] by auto
+  hence vderiv: "(D (\<lambda>t. \<phi> t s) = (\<lambda>t. f (\<phi> t s)) on {0<--<t + r/2})"
+    apply(rule has_vderiv_on_subset)
+    unfolding real_ivl_eqs[OF \<open>t + r/2 > 0\<close>] by auto
+  have "t \<in> {0<--<t + r/2}"
+    unfolding real_ivl_eqs[OF \<open>t + r/2 > 0\<close>] using rHyp \<open>t > 0\<close> by simp
+  moreover have "D (\<lambda>\<tau>. \<phi> \<tau> s) \<mapsto> (\<lambda>\<tau>. \<tau> *\<^sub>R f (\<phi> t s)) (at t within {0<--<t + r/2})"
+    using vderiv calculation unfolding has_vderiv_on_def has_vector_derivative_def by blast
+  moreover have "open {0<--<t + r/2}"
+    unfolding real_ivl_eqs[OF \<open>t + r/2 > 0\<close>] by simp
+  ultimately show ?thesis
+    using subs that by blast
+qed
+
+lemma has_derivative_on_open2: 
+  assumes "t < 0" "t \<in> T" "s \<in> S"
+  obtains B where "t \<in> B" and "open B" and "B \<subseteq> T"
+    and "D (\<lambda>\<tau>. \<phi> \<tau> s) \<mapsto> (\<lambda>\<tau>. \<tau> *\<^sub>R f (\<phi> t s)) at t within B" 
+proof-
+  obtain r::real where rHyp: "r > 0" "ball t r \<subseteq> T"
+    using open_contains_ball_eq open_domain(1) \<open>t \<in> T\<close> by blast
+  moreover have "t - r/2 < 0"
+    using \<open>r > 0\<close> \<open>t < 0\<close> by auto
+  moreover have "{0--t} \<subseteq> T" 
+    using subintervalI[OF init_time \<open>t \<in> T\<close>] .
+  ultimately have subs: "{0<--<t - r/2} \<subseteq> T"
+    unfolding open_segment_eq_real_ivl closed_segment_eq_real_ivl
+      real_ivl_eqs[OF rHyp(1)] by(auto simp: subset_eq)
+  have "t - r/2 \<in> T"
+    using rHyp unfolding real_ivl_eqs by (simp add: subset_eq)
+  hence "{0--t - r/2} \<subseteq> T"
+    using subintervalI[OF init_time] by blast
+  hence "(D (\<lambda>t. \<phi> t s) = (\<lambda>t. f (\<phi> t s)) on {0--(t - r/2)})"
+    using ivp(1)[OF _ \<open>s \<in> S\<close>] by auto
+  hence vderiv: "(D (\<lambda>t. \<phi> t s) = (\<lambda>t. f (\<phi> t s)) on {0<--<t - r/2})"
+    apply(rule has_vderiv_on_subset)
+    unfolding open_segment_eq_real_ivl closed_segment_eq_real_ivl by auto
+  have "t \<in> {0<--<t - r/2}"
+    unfolding open_segment_eq_real_ivl using rHyp \<open>t < 0\<close> by simp
+  moreover have "D (\<lambda>\<tau>. \<phi> \<tau> s) \<mapsto> (\<lambda>\<tau>. \<tau> *\<^sub>R f (\<phi> t s)) (at t within {0<--<t - r/2})"
+    using vderiv calculation unfolding has_vderiv_on_def has_vector_derivative_def by blast
+  moreover have "open {0<--<t - r/2}"
+    unfolding open_segment_eq_real_ivl by simp
+  ultimately show ?thesis
+    using subs that by blast
+qed
+
+lemma has_derivative_on_open3: 
+  assumes "s \<in> S"
+  obtains B where "0 \<in> B" and "open B" and "B \<subseteq> T"
+    and "D (\<lambda>\<tau>. \<phi> \<tau> s) \<mapsto> (\<lambda>\<tau>. \<tau> *\<^sub>R f (\<phi> 0 s)) at 0 within B" 
+proof-
+  obtain r::real where rHyp: "r > 0" "ball 0 r \<subseteq> T"
+    using open_contains_ball_eq open_domain(1) init_time by blast
+  hence "r/2 \<in> T" "-r/2 \<in> T" "r/2 > 0"
+    unfolding real_ivl_eqs by auto
+  hence subs: "{0--r/2} \<subseteq> T" "{0--(-r/2)} \<subseteq> T"
+    using subintervalI[OF init_time] by auto
+  hence "(D (\<lambda>t. \<phi> t s) = (\<lambda>t. f (\<phi> t s)) on {0--r/2})"
+    "(D (\<lambda>t. \<phi> t s) = (\<lambda>t. f (\<phi> t s)) on {0--(-r/2)})"
+    using ivp(1)[OF _ \<open>s \<in> S\<close>] by auto
+  also have "{0--r/2} = {0--r/2} \<union> closure {0--r/2} \<inter> closure {0--(-r/2)}"
+    "{0--(-r/2)} = {0--(-r/2)} \<union> closure {0--r/2} \<inter> closure {0--(-r/2)}"
+    unfolding closed_segment_eq_real_ivl \<open>r/2 > 0\<close> by auto
+  ultimately have vderivs:
+    "(D (\<lambda>t. \<phi> t s) = (\<lambda>t. f (\<phi> t s)) on {0--r/2} \<union> closure {0--r/2} \<inter> closure {0--(-r/2)})"
+    "(D (\<lambda>t. \<phi> t s) = (\<lambda>t. f (\<phi> t s)) on {0--(-r/2)} \<union> closure {0--r/2} \<inter> closure {0--(-r/2)})"
+    unfolding closed_segment_eq_real_ivl \<open>r/2 > 0\<close> by auto
+  have obs: "0 \<in> {-r/2<--<r/2}"
+    unfolding open_segment_eq_real_ivl using \<open>r/2 > 0\<close> by auto
+  have union: "{-r/2--r/2} = {0--r/2} \<union> {0--(-r/2)}"
+    unfolding closed_segment_eq_real_ivl by auto
+  hence "(D (\<lambda>t. \<phi> t s) = (\<lambda>t. f (\<phi> t s)) on {-r/2--r/2})"
+    using has_vderiv_on_union[OF vderivs] by simp
+  hence "(D (\<lambda>t. \<phi> t s) = (\<lambda>t. f (\<phi> t s)) on {-r/2<--<r/2})"
+    using has_vderiv_on_subset[OF _ segment_open_subset_closed[of "-r/2" "r/2"]] by auto
+  hence "D (\<lambda>\<tau>. \<phi> \<tau> s) \<mapsto> (\<lambda>\<tau>. \<tau> *\<^sub>R f (\<phi> 0 s)) (at 0 within {-r/2<--<r/2})"
+    unfolding has_vderiv_on_def has_vector_derivative_def using obs by blast
+  moreover have "open {-r/2<--<r/2}"
+    unfolding open_segment_eq_real_ivl by simp
+  moreover have "{-r/2<--<r/2} \<subseteq> T"
+    using subs union segment_open_subset_closed by blast 
+  ultimately show ?thesis
+    using obs that by blast
+qed
+
+lemma has_derivative_on_open: 
+  assumes "t \<in> T" "s \<in> S"
+  obtains B where "t \<in> B" and "open B" and "B \<subseteq> T"
+    and "D (\<lambda>\<tau>. \<phi> \<tau> s) \<mapsto> (\<lambda>\<tau>. \<tau> *\<^sub>R f (\<phi> t s)) at t within B" 
+  apply(subgoal_tac "t < 0 \<or> t = 0 \<or> t > 0")
+  using has_derivative_on_open1[OF _ assms] has_derivative_on_open2[OF _ assms]
+    has_derivative_on_open3[OF \<open>s \<in> S\<close>] by blast force
+
+lemma has_vderiv_on_domain:
+  assumes "s \<in> S"
+  shows "D (\<lambda>t. \<phi> t s) = (\<lambda>t. f (\<phi> t s)) on T"
+proof(unfold has_vderiv_on_def has_vector_derivative_def, clarsimp)
+  fix t assume "t \<in> T"
+  then obtain B where "t \<in> B" and "open B" and "B \<subseteq> T" 
+    and Dhyp: "D (\<lambda>t. \<phi> t s) \<mapsto> (\<lambda>xa. xa *\<^sub>R f (\<phi> t s)) at t within B"
+    using assms has_derivative_on_open[OF \<open>t \<in> T\<close>] by blast
+  hence "t \<in> interior B"
+    using interior_eq by auto
+  thus "D (\<lambda>t. \<phi> t s) \<mapsto> (\<lambda>xa. xa *\<^sub>R f (\<phi> t s)) at t within T"
+    using has_derivative_at_within_mono[OF _ \<open>B \<subseteq> T\<close> Dhyp] by blast
+qed
+
+lemma eq_solution:
+  assumes "X \<in> (ivp_sols (\<lambda>t. f) T S 0 s)" and "t \<in> T" and "s \<in> S"
+  shows "X t = \<phi> t s"
+proof-
+  have "D X = (\<lambda>t. f (X t)) on (ex_ivl s)" and "X 0 = s" and "X \<in> (ex_ivl s) \<rightarrow> S"
+    using ivp_solsD[OF assms(1)] unfolding ex_ivl_eq[OF \<open>s \<in> S\<close>] by auto
+  note solution_eq_flow[OF this]
+  hence "X t = flow 0 s t"
+    unfolding ex_ivl_eq[OF \<open>s \<in> S\<close>] using assms by blast
+  also have "\<phi> t s = flow 0 s t"
+    apply(rule solution_eq_flow ivp)
+        apply(simp_all add: assms(2,3) ivp(2)[OF \<open>s \<in> S\<close>])
+    unfolding ex_ivl_eq[OF \<open>s \<in> S\<close>] by (auto simp: has_vderiv_on_domain assms in_domain)
+  ultimately show "X t = \<phi> t s"
+    by simp
+qed
+
+lemma in_ivp_sols: 
+  assumes "s \<in> S"
+  shows "(\<lambda>t. \<phi> t s) \<in> ivp_sols (\<lambda>t. f) T S 0 s"
+  using has_vderiv_on_domain ivp(2) in_domain apply(rule ivp_solsI)
+  using assms by auto
+
+lemma eq_solution_ivl:
+  assumes xivp: "D X = (\<lambda>t. f (X t)) on {0--t}" "X 0 = s" "X \<in> {0--t} \<rightarrow> S" 
+    and indom: "t \<in> T" "s \<in> S"
+  shows "X t = \<phi> t s"
+  apply(rule unique_solution[OF xivp \<open>t \<in> T\<close>])
+  using \<open>s \<in> S\<close> ivp indom by auto
+
+lemma additive_in_ivp_sols:
+  assumes "s \<in> S" and "(\<lambda>\<tau>. \<tau> + t) ` T \<subseteq> T"
+  shows "(\<lambda>\<tau>. \<phi> (\<tau> + t) s) \<in> ivp_sols (\<lambda>t. f) T S 0 (\<phi> (0 + t) s)"
+  apply(rule ivp_solsI, rule vderiv_on_compose_add)
+  using has_vderiv_on_domain has_vderiv_on_subset assms apply blast
+  using in_domain assms by auto
+
+lemma is_monoid_action:
+  assumes indom: "t\<^sub>1 \<in> T" "t\<^sub>2 \<in> T" "s \<in> S" 
+    and "(\<lambda>\<tau>. \<tau> + t\<^sub>2) ` T \<subseteq> T"
+  shows "\<phi> 0 s = s"
+    and "\<phi> (t\<^sub>1 + t\<^sub>2) s = \<phi> t\<^sub>1 (\<phi> t\<^sub>2 s)"
+proof-
+  show "\<phi> 0 s = s"
+    using ivp indom by simp
+  have "\<phi> (0 + t\<^sub>2) s = \<phi> t\<^sub>2 s" 
+    by simp
+  also have "\<phi> t\<^sub>2 s \<in> S"
+    using in_domain indom by auto
+  finally show "\<phi> (t\<^sub>1 + t\<^sub>2) s = \<phi> t\<^sub>1 (\<phi> t\<^sub>2 s)"
+    using eq_solution[OF additive_in_ivp_sols] assms by auto
+qed
+
+lemma orbit_eq[simp]: 
+  assumes "s \<in> S"
+  shows "\<gamma>\<^sup>\<phi> s = {\<phi> t s| t. t \<in> T}"
+  using eq_solution assms unfolding orbit_def g_orbital_eq ivp_sols_def
+  by(auto intro!: has_vderiv_on_domain ivp(2) in_domain)
+
+lemma g_orbit_eq: 
+  assumes "s \<in> S"
+  shows "\<gamma>\<^sup>\<phi>\<^sub>G\<^sub>u\<^sub>a\<^sub>r\<^sub>d G s = {\<phi> t s| t. t \<in> T \<and> G \<rhd> (\<lambda>r. \<phi> r s) (down T t)}" (is "_ = ?gorbit")
+proof(rule subset_antisym, simp_all only: subset_eq)
+  {fix s' assume "s' \<in> \<gamma>\<^sup>\<phi>\<^sub>G\<^sub>u\<^sub>a\<^sub>r\<^sub>d G s"
+    then obtain x and t where x_ivp:"x \<in> ivp_sols (\<lambda>t. f) T S 0 s" 
+      and "x t = s'" and "t \<in> T" and guard:"G \<rhd> x (down T t)"
+      unfolding g_orbital_def by auto
+    hence obs:"\<forall>\<tau>\<in>(down T t). x \<tau> = \<phi> \<tau> s"
+      using eq_solution[OF x_ivp _ assms] init_time
+      by blast
+    hence "G \<rhd> (\<lambda>r. \<phi> r s) (down T t)"
+      using guard
+      by auto 
+    also have "\<phi> t s = x t"
+      using eq_solution[OF x_ivp \<open>t \<in> T\<close> assms] by simp
+    ultimately have "s' \<in> ?gorbit"
+      using \<open>x t = s'\<close> \<open>t \<in> T\<close> by auto}
+  thus "\<forall>s'\<in>\<gamma>\<^sup>\<phi>\<^sub>G\<^sub>u\<^sub>a\<^sub>r\<^sub>d G s. s' \<in> ?gorbit"
+    by blast
+next
+  {fix s' assume "s' \<in> ?gorbit"
+    then obtain t where "G \<rhd> (\<lambda>r. \<phi> r s) (down T t)" and "t \<in> T" and "\<phi> t s = s'"
+      by blast
+    hence "s' \<in> \<gamma>\<^sup>\<phi>\<^sub>G\<^sub>u\<^sub>a\<^sub>r\<^sub>d G s"
+      using assms by(auto intro!: g_orbitalI in_domain ivp(2) 
+          has_vderiv_on_domain simp: init_time)}
+  thus "\<forall>s'\<in>?gorbit. s' \<in> \<gamma>\<^sup>\<phi>\<^sub>G\<^sub>u\<^sub>a\<^sub>r\<^sub>d G s"
+    by blast
+qed
+
+lemma ivp_sols_collapse: 
+  assumes "S = UNIV" "T = UNIV"
+  shows "ivp_sols (\<lambda>t. f) T S 0 s = {(\<lambda>t. \<phi> t s)}"
+  using in_ivp_sols eq_solution unfolding assms by auto
+
+lemma diff_invariant_eq_invariant_set:
+  "(I is_diff_invariant_of f along T S from 0) = (\<forall>s\<in>S. \<forall>t\<in>T. I s \<longrightarrow> I (\<phi> t s))"
+  apply(subst invariant_to_set, safe)
+   apply(erule_tac x=s in ballE)
+  unfolding g_orbit_eq by auto
+
+end
+
+end
